specs/tests/Spec.HPKE.Test.fst
@@ -16,797 +16,1980 @@ module HKDF = Spec.Agile.HKDF
 
 friend Spec.Agile.HPKE
 
-// Test1: A.1, DHKEM(Curve25519), HKDF-SHA256, AES-GCM-128
-// Base Setup
-// mode: 0
-// kemID: 2
-// kdfID: 1
-// aeadID: 1
-// info: 4f6465206f6e2061204772656369616e2055726e
-// skR: 39516b2f05e9757e21331c6f2019045f52cee01a741e2a8b50380408d0717fd9
-// skS: eea949550bb218c921ab85cbc5003f4ef6257db1b47b7ed63a223c8360ef81e3
-// skE: a1f7746c45d1a0eb72b996e0e7ecddba0e60a583a5e143796981101a3aaf8966
-// psk: 3564623362383061383163623633636135393437306338333431346566373061633
-// 1636338303636333964303133353738343937343061303364616464666339
-// pskID: 456e6e796e20447572696e206172616e204d6f726961
-// pkR: 14fdb807c79fb787d47890d502bce7c335d0809a053b9287e30fc608fcfc9d26
-// pkS: 6eac89bc5d63e7b40c394a4218b6a8203803749f95fca2369611ed41afb97e06
-// pkE: 0454a5a10ecaf982219eae4b5c36bc3e1606813caae1d262528396c60de44e3d
-// enc: 0454a5a10ecaf982219eae4b5c36bc3e1606813caae1d262528396c60de44e3d
-// zz: 15178ef77262b0468ee828a6da4f2620434a9edfdddfe9256ac53f8c6b7e575d
-// context: 000002000100010454a5a10ecaf982219eae4b5c36bc3e1606813caae1d2625
-// 28396c60de44e3d14fdb807c79fb787d47890d502bce7c335d0809a053b9287e30fc608f
-// cfc9d260000000000000000000000000000000000000000000000000000000000000000e
-// 3b0c44298fc1c149afbf4c8996fb92427ae41e4649b934ca495991b7852b85555c404062
-// 9c64c5efec2f7230407d612d16289d7c5d7afcf9340280abd2de1ab
-// secret: c5fdbbad5c72ed703581bbcd3fe890a7ed46d6bf00c73c9755bffbcd6744f22b
-// key: 11cf34f93b3d1e8f2e36f91c5a2d6818
-// nonce: 23acef669d7f3bcc98f6d0ab
+let print (str:string) =
+  IO.print_string str
 
-// sequence number: 0
-// plaintext: 4265617574792069732074727574682c20747275746820626561757479
-// aad: 436f756e742d30
-// nonce: 23acef669d7f3bcc98f6d0ab
-// ciphertext: 13fc68aef8e2c4591a0dd92c01ffe9573314d881cf71dd5708644ee71848
-// 18e457de3b4d51eb1deb4f0beb35d1
+#set-options "--z3rlimit 100 --fuel 0 --ifuel 1"
+let print_bytes (prefix:string) (len:size_nat) (bytes:lbytes len) =
+  print prefix;
+  List.iter (fun a -> print (UInt8.to_string (u8_to_UInt8 a))) (to_list bytes)
 
-// sequence number: 1
-// plaintext: 4265617574792069732074727574682c20747275746820626561757479
-// aad: 436f756e742d31
-// nonce: 23acef669d7f3bcc98f6d0aa
-// ciphertext: 2d7f0e514ce14abf93b0fcc34347e20d23008465c6f98aedc1f1fa806bfc
-// 07708ff20ae9989bb770b18493f3af
+let compare_bytes (len:size_nat) (test_expected:lbytes len) (test_result:lbytes len) =
+  for_all2 (fun a b -> uint_to_nat #U8 a = uint_to_nat #U8 b) test_expected test_result
 
-// sequence number: 2
-// plaintext: 4265617574792069732074727574682c20747275746820626561757479
-// aad: 436f756e742d32
-// nonce: 23acef669d7f3bcc98f6d0a9
-// ciphertext: 3fa07d648ba64a5dd3816c2a512937c2a58b8428a1067b5ac15841541d5c
-// 6d28cd415faba7d552d606d6c5f48c
+let print_and_compare_bytes (len:size_nat) (test_expected:lbytes len) (test_result:lbytes len) =
+  print_bytes "Result:   " len test_result;
+  print "\n";
+  print_bytes "Expected: " len test_expected;
+  print "\n";
+  compare_bytes len test_expected test_result
 
-// sequence number: 4
-// plaintext: 4265617574792069732074727574682c20747275746820626561757479
-// aad: 436f756e742d34
-// nonce: 23acef669d7f3bcc98f6d0af
-// ciphertext: 3aeeea18f990589141df055a90f382a8096dbdae8f912291cfeff475ede4
-// f9b023c3ce88f499f5a2dc44454241
+let test1_mode: HPKE.mode = HPKE.Base
+let test1_ciphersuite = DH.DH_Curve25519, Hash.SHA2_256, AEAD.AES128_GCM, Hash.SHA2_256
 
-let test1_ciphersuite = DH.DH_Curve25519, AEAD.AES128_GCM, Hash.SHA2_256
+// generated: "4f6465206f6e2061204772656369616e2055726e"
+inline_for_extraction
+let size_test1_info: size_nat = 20
+let test1_info_list : l:list uint8{List.Tot.length l == size_test1_info} =
+  [@inline_let]
+  let l = [
+    u8 0x4f; u8 0x64; u8 0x65; u8 0x20; u8 0x6f;
+    u8 0x6e; u8 0x20; u8 0x61; u8 0x20; u8 0x47;
+    u8 0x72; u8 0x65; u8 0x63; u8 0x69; u8 0x61;
+    u8 0x6e; u8 0x20; u8 0x55; u8 0x72; u8 0x6e;
+  ] in
+  assert_norm(List.Tot.length l == size_test1_info);
+  l
+let test1_info : lbytes size_test1_info = createL test1_info_list
 
-let test1_info = List.Tot.map u8_from_UInt8 [
-  0x4fuy; 0x64uy; 0x65uy; 0x20uy; 0x6fuy;
-  0x6euy; 0x20uy; 0x61uy; 0x20uy; 0x47uy;
-  0x72uy; 0x65uy; 0x63uy; 0x69uy; 0x61uy;
-  0x6euy; 0x20uy; 0x55uy; 0x72uy; 0x6euy
-]
+// generated: "919f0e1b7c361d1e5a3d0086ba94edeb6d2df9f756654741731f4e84cb813bdb"
+inline_for_extraction
+let size_test1_skRm: size_nat = 32
+let test1_skRm_list : l:list uint8{List.Tot.length l == size_test1_skRm} =
+  [@inline_let]
+  let l = [
+    u8 0x91; u8 0x9f; u8 0x0e; u8 0x1b; u8 0x7c;
+    u8 0x36; u8 0x1d; u8 0x1e; u8 0x5a; u8 0x3d;
+    u8 0x00; u8 0x86; u8 0xba; u8 0x94; u8 0xed;
+    u8 0xeb; u8 0x6d; u8 0x2d; u8 0xf9; u8 0xf7;
+    u8 0x56; u8 0x65; u8 0x47; u8 0x41; u8 0x73;
+    u8 0x1f; u8 0x4e; u8 0x84; u8 0xcb; u8 0x81;
+    u8 0x3b; u8 0xdb;
+  ] in
+  assert_norm(List.Tot.length l == size_test1_skRm);
+  l
+let test1_skRm : lbytes size_test1_skRm = createL test1_skRm_list
 
-let test1_skR = List.Tot.map u8_from_UInt8 [
-  0x39uy; 0x51uy; 0x6buy; 0x2fuy; 0x05uy;
-  0xe9uy; 0x75uy; 0x7euy; 0x21uy; 0x33uy;
-  0x1cuy; 0x6fuy; 0x20uy; 0x19uy; 0x04uy;
-  0x5fuy; 0x52uy; 0xceuy; 0xe0uy; 0x1auy;
-  0x74uy; 0x1euy; 0x2auy; 0x8buy; 0x50uy;
-  0x38uy; 0x04uy; 0x08uy; 0xd0uy; 0x71uy;
-  0x7fuy; 0xd9uy;
-]
+// generated: "232ce0da9fd45b8d500781a5ee1b0a2cf64411dd08d6442400ab05a4d29733a8"
+inline_for_extraction
+let size_test1_skEm: size_nat = 32
+let test1_skEm_list : l:list uint8{List.Tot.length l == size_test1_skEm} =
+  [@inline_let]
+  let l = [
+    u8 0x23; u8 0x2c; u8 0xe0; u8 0xda; u8 0x9f;
+    u8 0xd4; u8 0x5b; u8 0x8d; u8 0x50; u8 0x07;
+    u8 0x81; u8 0xa5; u8 0xee; u8 0x1b; u8 0x0a;
+    u8 0x2c; u8 0xf6; u8 0x44; u8 0x11; u8 0xdd;
+    u8 0x08; u8 0xd6; u8 0x44; u8 0x24; u8 0x00;
+    u8 0xab; u8 0x05; u8 0xa4; u8 0xd2; u8 0x97;
+    u8 0x33; u8 0xa8;
+  ] in
+  assert_norm(List.Tot.length l == size_test1_skEm);
+  l
+let test1_skEm : lbytes size_test1_skEm = createL test1_skEm_list
 
-let test1_skI = List.Tot.map u8_from_UInt8 [
-  0xeeuy; 0xa9uy; 0x49uy; 0x55uy; 0x0buy;
-  0xb2uy; 0x18uy; 0xc9uy; 0x21uy; 0xabuy;
-  0x85uy; 0xcbuy; 0xc5uy; 0x00uy; 0x3fuy;
-  0x4euy; 0xf6uy; 0x25uy; 0x7duy; 0xb1uy;
-  0xb4uy; 0x7buy; 0x7euy; 0xd6uy; 0x3auy;
-  0x22uy; 0x3cuy; 0x83uy; 0x60uy; 0xefuy;
-  0x81uy; 0xe3uy;
-]
+// generated: "ac511615dee12b2e11170f1272c3972e6e2268d8fb05fc93c6b008065f61f22f"
+inline_for_extraction
+let size_test1_pkRm: size_nat = 32
+let test1_pkRm_list : l:list uint8{List.Tot.length l == size_test1_pkRm} =
+  [@inline_let]
+  let l = [
+    u8 0xac; u8 0x51; u8 0x16; u8 0x15; u8 0xde;
+    u8 0xe1; u8 0x2b; u8 0x2e; u8 0x11; u8 0x17;
+    u8 0x0f; u8 0x12; u8 0x72; u8 0xc3; u8 0x97;
+    u8 0x2e; u8 0x6e; u8 0x22; u8 0x68; u8 0xd8;
+    u8 0xfb; u8 0x05; u8 0xfc; u8 0x93; u8 0xc6;
+    u8 0xb0; u8 0x08; u8 0x06; u8 0x5f; u8 0x61;
+    u8 0xf2; u8 0x2f;
+  ] in
+  assert_norm(List.Tot.length l == size_test1_pkRm);
+  l
+let test1_pkRm : lbytes size_test1_pkRm = createL test1_pkRm_list
 
-let test1_skE = List.Tot.map u8_from_UInt8 [
-  0xa1uy; 0xf7uy; 0x74uy; 0x6cuy; 0x45uy;
-  0xd1uy; 0xa0uy; 0xebuy; 0x72uy; 0xb9uy;
-  0x96uy; 0xe0uy; 0xe7uy; 0xecuy; 0xdduy;
-  0xbauy; 0x0euy; 0x60uy; 0xa5uy; 0x83uy;
-  0xa5uy; 0xe1uy; 0x43uy; 0x79uy; 0x69uy;
-  0x81uy; 0x10uy; 0x1auy; 0x3auy; 0xafuy;
-  0x89uy; 0x66uy;
-]
+// generated: "ab8b7fdda7ed10c410079909350948ff63bc044b40575cc85636f3981bb8d258"
+inline_for_extraction
+let size_test1_pkEm: size_nat = 32
+let test1_pkEm_list : l:list uint8{List.Tot.length l == size_test1_pkEm} =
+  [@inline_let]
+  let l = [
+    u8 0xab; u8 0x8b; u8 0x7f; u8 0xdd; u8 0xa7;
+    u8 0xed; u8 0x10; u8 0xc4; u8 0x10; u8 0x07;
+    u8 0x99; u8 0x09; u8 0x35; u8 0x09; u8 0x48;
+    u8 0xff; u8 0x63; u8 0xbc; u8 0x04; u8 0x4b;
+    u8 0x40; u8 0x57; u8 0x5c; u8 0xc8; u8 0x56;
+    u8 0x36; u8 0xf3; u8 0x98; u8 0x1b; u8 0xb8;
+    u8 0xd2; u8 0x58;
+  ] in
+  assert_norm(List.Tot.length l == size_test1_pkEm);
+  l
+let test1_pkEm : lbytes size_test1_pkEm = createL test1_pkEm_list
 
-let test1_psk = List.Tot.map u8_from_UInt8 [
-  0x35uy; 0x64uy; 0x62uy; 0x33uy; 0x62uy;
-  0x38uy; 0x30uy; 0x61uy; 0x38uy; 0x31uy;
-  0x63uy; 0x62uy; 0x36uy; 0x33uy; 0x63uy;
-  0x61uy; 0x35uy; 0x39uy; 0x34uy; 0x37uy;
-  0x30uy; 0x63uy; 0x38uy; 0x33uy; 0x34uy;
-  0x31uy; 0x34uy; 0x65uy; 0x66uy; 0x37uy;
-  0x30uy; 0x61uy; 0x63uy; 0x31uy; 0x63uy;
-  0x63uy; 0x38uy; 0x30uy; 0x36uy; 0x36uy;
-  0x33uy; 0x39uy; 0x64uy; 0x30uy; 0x31uy;
-  0x33uy; 0x35uy; 0x37uy; 0x38uy; 0x34uy;
-  0x39uy; 0x37uy; 0x34uy; 0x30uy; 0x61uy;
-  0x30uy; 0x33uy; 0x64uy; 0x61uy; 0x64uy;
-  0x64uy; 0x66uy; 0x63uy; 0x39uy;
-]
+// generated: "ab8b7fdda7ed10c410079909350948ff63bc044b40575cc85636f3981bb8d258"
+inline_for_extraction
+let size_test1_enc: size_nat = 32
+let test1_enc_list : l:list uint8{List.Tot.length l == size_test1_enc} =
+  [@inline_let]
+  let l = [
+    u8 0xab; u8 0x8b; u8 0x7f; u8 0xdd; u8 0xa7;
+    u8 0xed; u8 0x10; u8 0xc4; u8 0x10; u8 0x07;
+    u8 0x99; u8 0x09; u8 0x35; u8 0x09; u8 0x48;
+    u8 0xff; u8 0x63; u8 0xbc; u8 0x04; u8 0x4b;
+    u8 0x40; u8 0x57; u8 0x5c; u8 0xc8; u8 0x56;
+    u8 0x36; u8 0xf3; u8 0x98; u8 0x1b; u8 0xb8;
+    u8 0xd2; u8 0x58;
+  ] in
+  assert_norm(List.Tot.length l == size_test1_enc);
+  l
+let test1_enc : lbytes size_test1_enc = createL test1_enc_list
+
+// generated: "44807c99177b0f3761d66f422945a21317a1532ca038e976594487a6a7e58fbf"
+inline_for_extraction
+let size_test1_zz: size_nat = 32
+let test1_zz_list : l:list uint8{List.Tot.length l == size_test1_zz} =
+  [@inline_let]
+  let l = [
+    u8 0x44; u8 0x80; u8 0x7c; u8 0x99; u8 0x17;
+    u8 0x7b; u8 0x0f; u8 0x37; u8 0x61; u8 0xd6;
+    u8 0x6f; u8 0x42; u8 0x29; u8 0x45; u8 0xa2;
+    u8 0x13; u8 0x17; u8 0xa1; u8 0x53; u8 0x2c;
+    u8 0xa0; u8 0x38; u8 0xe9; u8 0x76; u8 0x59;
+    u8 0x44; u8 0x87; u8 0xa6; u8 0xa7; u8 0xe5;
+    u8 0x8f; u8 0xbf;
+  ] in
+  assert_norm(List.Tot.length l == size_test1_zz);
+  l
+let test1_zz : lbytes size_test1_zz = createL test1_zz_list
+
+// generated: "002000010001005d0f5548cb13d7eba5320ae0e21b1ee274aac7ea1cce02570cf993d1b2456449debcca602075cf6f8ef506613a82e1c73727e2c912d0c49f16cd56fc524af4ce"
+inline_for_extraction
+let size_test1_key_schedule_context: size_nat = 71
+let test1_key_schedule_context_list : l:list uint8{List.Tot.length l == size_test1_key_schedule_context} =
+  [@inline_let]
+  let l = [
+    u8 0x00; u8 0x20; u8 0x00; u8 0x01; u8 0x00;
+    u8 0x01; u8 0x00; u8 0x5d; u8 0x0f; u8 0x55;
+    u8 0x48; u8 0xcb; u8 0x13; u8 0xd7; u8 0xeb;
+    u8 0xa5; u8 0x32; u8 0x0a; u8 0xe0; u8 0xe2;
+    u8 0x1b; u8 0x1e; u8 0xe2; u8 0x74; u8 0xaa;
+    u8 0xc7; u8 0xea; u8 0x1c; u8 0xce; u8 0x02;
+    u8 0x57; u8 0x0c; u8 0xf9; u8 0x93; u8 0xd1;
+    u8 0xb2; u8 0x45; u8 0x64; u8 0x49; u8 0xde;
+    u8 0xbc; u8 0xca; u8 0x60; u8 0x20; u8 0x75;
+    u8 0xcf; u8 0x6f; u8 0x8e; u8 0xf5; u8 0x06;
+    u8 0x61; u8 0x3a; u8 0x82; u8 0xe1; u8 0xc7;
+    u8 0x37; u8 0x27; u8 0xe2; u8 0xc9; u8 0x12;
+    u8 0xd0; u8 0xc4; u8 0x9f; u8 0x16; u8 0xcd;
+    u8 0x56; u8 0xfc; u8 0x52; u8 0x4a; u8 0xf4;
+    u8 0xce;
+  ] in
+  assert_norm(List.Tot.length l == size_test1_key_schedule_context);
+  l
+let test1_key_schedule_context : lbytes size_test1_key_schedule_context = createL test1_key_schedule_context_list
+
+// generated: "c104521df56de97b517165011f09e0ea2a36b9af339a9de402c8b88547c8b67e"
+inline_for_extraction
+let size_test1_secret: size_nat = 32
+let test1_secret_list : l:list uint8{List.Tot.length l == size_test1_secret} =
+  [@inline_let]
+  let l = [
+    u8 0xc1; u8 0x04; u8 0x52; u8 0x1d; u8 0xf5;
+    u8 0x6d; u8 0xe9; u8 0x7b; u8 0x51; u8 0x71;
+    u8 0x65; u8 0x01; u8 0x1f; u8 0x09; u8 0xe0;
+    u8 0xea; u8 0x2a; u8 0x36; u8 0xb9; u8 0xaf;
+    u8 0x33; u8 0x9a; u8 0x9d; u8 0xe4; u8 0x02;
+    u8 0xc8; u8 0xb8; u8 0x85; u8 0x47; u8 0xc8;
+    u8 0xb6; u8 0x7e;
+  ] in
+  assert_norm(List.Tot.length l == size_test1_secret);
+  l
+let test1_secret : lbytes size_test1_secret = createL test1_secret_list
+
+// generated: "e34afc8f8f4c2906b310d8e4e4d526f0"
+inline_for_extraction
+let size_test1_key: size_nat = 16
+let test1_key_list : l:list uint8{List.Tot.length l == size_test1_key} =
+  [@inline_let]
+  let l = [
+    u8 0xe3; u8 0x4a; u8 0xfc; u8 0x8f; u8 0x8f;
+    u8 0x4c; u8 0x29; u8 0x06; u8 0xb3; u8 0x10;
+    u8 0xd8; u8 0xe4; u8 0xe4; u8 0xd5; u8 0x26;
+    u8 0xf0;
+  ] in
+  assert_norm(List.Tot.length l == size_test1_key);
+  l
+let test1_key : lbytes size_test1_key = createL test1_key_list
+
+// generated: "2764228860619e140920c7d7"
+inline_for_extraction
+let size_test1_nonce: size_nat = 12
+let test1_nonce_list : l:list uint8{List.Tot.length l == size_test1_nonce} =
+  [@inline_let]
+  let l = [
+    u8 0x27; u8 0x64; u8 0x22; u8 0x88; u8 0x60;
+    u8 0x61; u8 0x9e; u8 0x14; u8 0x09; u8 0x20;
+    u8 0xc7; u8 0xd7;
+  ] in
+  assert_norm(List.Tot.length l == size_test1_nonce);
+  l
+let test1_nonce : lbytes size_test1_nonce = createL test1_nonce_list
+
+// generated: "93c6a28ec7af55f669612d5d64fe680ae38ca88d14fb6ecba647606eee668124"
+inline_for_extraction
+let size_test1_exporterSecret: size_nat = 32
+let test1_exporterSecret_list : l:list uint8{List.Tot.length l == size_test1_exporterSecret} =
+  [@inline_let]
+  let l = [
+    u8 0x93; u8 0xc6; u8 0xa2; u8 0x8e; u8 0xc7;
+    u8 0xaf; u8 0x55; u8 0xf6; u8 0x69; u8 0x61;
+    u8 0x2d; u8 0x5d; u8 0x64; u8 0xfe; u8 0x68;
+    u8 0x0a; u8 0xe3; u8 0x8c; u8 0xa8; u8 0x8d;
+    u8 0x14; u8 0xfb; u8 0x6e; u8 0xcb; u8 0xa6;
+    u8 0x47; u8 0x60; u8 0x6e; u8 0xee; u8 0x66;
+    u8 0x81; u8 0x24;
+  ] in
+  assert_norm(List.Tot.length l == size_test1_exporterSecret);
+  l
+let test1_exporterSecret : lbytes size_test1_exporterSecret = createL test1_exporterSecret_list
+
+// generated: "436f756e742d30"
+inline_for_extraction
+let size_test1_encryption0_aad: size_nat = 7
+let test1_encryption0_aad_list : l:list uint8{List.Tot.length l == size_test1_encryption0_aad} =
+  [@inline_let]
+  let l = [
+    u8 0x43; u8 0x6f; u8 0x75; u8 0x6e; u8 0x74;
+    u8 0x2d; u8 0x30;
+  ] in
+  assert_norm(List.Tot.length l == size_test1_encryption0_aad);
+  l
+let test1_encryption0_aad : lbytes size_test1_encryption0_aad = createL test1_encryption0_aad_list
+
+// generated: "1811cf5d39f857f80175f96ca4d3600bfb0585e4ce119bc46396da4b371966a358924e5a97a7b53ea255971f6b"
+inline_for_extraction
+let size_test1_encryption0_ciphertext: size_nat = 45
+let test1_encryption0_ciphertext_list : l:list uint8{List.Tot.length l == size_test1_encryption0_ciphertext} =
+  [@inline_let]
+  let l = [
+    u8 0x18; u8 0x11; u8 0xcf; u8 0x5d; u8 0x39;
+    u8 0xf8; u8 0x57; u8 0xf8; u8 0x01; u8 0x75;
+    u8 0xf9; u8 0x6c; u8 0xa4; u8 0xd3; u8 0x60;
+    u8 0x0b; u8 0xfb; u8 0x05; u8 0x85; u8 0xe4;
+    u8 0xce; u8 0x11; u8 0x9b; u8 0xc4; u8 0x63;
+    u8 0x96; u8 0xda; u8 0x4b; u8 0x37; u8 0x19;
+    u8 0x66; u8 0xa3; u8 0x58; u8 0x92; u8 0x4e;
+    u8 0x5a; u8 0x97; u8 0xa7; u8 0xb5; u8 0x3e;
+    u8 0xa2; u8 0x55; u8 0x97; u8 0x1f; u8 0x6b;
+  ] in
+  assert_norm(List.Tot.length l == size_test1_encryption0_ciphertext);
+  l
+let test1_encryption0_ciphertext : lbytes size_test1_encryption0_ciphertext = createL test1_encryption0_ciphertext_list
+
+// generated: "2764228860619e140920c7d7"
+inline_for_extraction
+let size_test1_encryption0_nonce: size_nat = 12
+let test1_encryption0_nonce_list : l:list uint8{List.Tot.length l == size_test1_encryption0_nonce} =
+  [@inline_let]
+  let l = [
+    u8 0x27; u8 0x64; u8 0x22; u8 0x88; u8 0x60;
+    u8 0x61; u8 0x9e; u8 0x14; u8 0x09; u8 0x20;
+    u8 0xc7; u8 0xd7;
+  ] in
+  assert_norm(List.Tot.length l == size_test1_encryption0_nonce);
+  l
+let test1_encryption0_nonce : lbytes size_test1_encryption0_nonce = createL test1_encryption0_nonce_list
+
+// generated: "4265617574792069732074727574682c20747275746820626561757479"
+inline_for_extraction
+let size_test1_encryption0_plaintext: size_nat = 29
+let test1_encryption0_plaintext_list : l:list uint8{List.Tot.length l == size_test1_encryption0_plaintext} =
+  [@inline_let]
+  let l = [
+    u8 0x42; u8 0x65; u8 0x61; u8 0x75; u8 0x74;
+    u8 0x79; u8 0x20; u8 0x69; u8 0x73; u8 0x20;
+    u8 0x74; u8 0x72; u8 0x75; u8 0x74; u8 0x68;
+    u8 0x2c; u8 0x20; u8 0x74; u8 0x72; u8 0x75;
+    u8 0x74; u8 0x68; u8 0x20; u8 0x62; u8 0x65;
+    u8 0x61; u8 0x75; u8 0x74; u8 0x79;
+  ] in
+  assert_norm(List.Tot.length l == size_test1_encryption0_plaintext);
+  l
+let test1_encryption0_plaintext : lbytes size_test1_encryption0_plaintext = createL test1_encryption0_plaintext_list
+
+// generated: "436f756e742d31"
+inline_for_extraction
+let size_test1_encryption1_aad: size_nat = 7
+let test1_encryption1_aad_list : l:list uint8{List.Tot.length l == size_test1_encryption1_aad} =
+  [@inline_let]
+  let l = [
+    u8 0x43; u8 0x6f; u8 0x75; u8 0x6e; u8 0x74;
+    u8 0x2d; u8 0x31;
+  ] in
+  assert_norm(List.Tot.length l == size_test1_encryption1_aad);
+  l
+let test1_encryption1_aad : lbytes size_test1_encryption1_aad = createL test1_encryption1_aad_list
+
+// generated: "2ed9ff66c33bad2f7c0326881f05aa9616ccba13bdb126a0d2a5a3dfa6b95bd4de78a98ff64c1fb64b366074d4"
+inline_for_extraction
+let size_test1_encryption1_ciphertext: size_nat = 45
+let test1_encryption1_ciphertext_list : l:list uint8{List.Tot.length l == size_test1_encryption1_ciphertext} =
+  [@inline_let]
+  let l = [
+    u8 0x2e; u8 0xd9; u8 0xff; u8 0x66; u8 0xc3;
+    u8 0x3b; u8 0xad; u8 0x2f; u8 0x7c; u8 0x03;
+    u8 0x26; u8 0x88; u8 0x1f; u8 0x05; u8 0xaa;
+    u8 0x96; u8 0x16; u8 0xcc; u8 0xba; u8 0x13;
+    u8 0xbd; u8 0xb1; u8 0x26; u8 0xa0; u8 0xd2;
+    u8 0xa5; u8 0xa3; u8 0xdf; u8 0xa6; u8 0xb9;
+    u8 0x5b; u8 0xd4; u8 0xde; u8 0x78; u8 0xa9;
+    u8 0x8f; u8 0xf6; u8 0x4c; u8 0x1f; u8 0xb6;
+    u8 0x4b; u8 0x36; u8 0x60; u8 0x74; u8 0xd4;
+  ] in
+  assert_norm(List.Tot.length l == size_test1_encryption1_ciphertext);
+  l
+let test1_encryption1_ciphertext : lbytes size_test1_encryption1_ciphertext = createL test1_encryption1_ciphertext_list
+
+// generated: "2764228860619e140920c7d6"
+inline_for_extraction
+let size_test1_encryption1_nonce: size_nat = 12
+let test1_encryption1_nonce_list : l:list uint8{List.Tot.length l == size_test1_encryption1_nonce} =
+  [@inline_let]
+  let l = [
+    u8 0x27; u8 0x64; u8 0x22; u8 0x88; u8 0x60;
+    u8 0x61; u8 0x9e; u8 0x14; u8 0x09; u8 0x20;
+    u8 0xc7; u8 0xd6;
+  ] in
+  assert_norm(List.Tot.length l == size_test1_encryption1_nonce);
+  l
+let test1_encryption1_nonce : lbytes size_test1_encryption1_nonce = createL test1_encryption1_nonce_list
+
+// generated: "4265617574792069732074727574682c20747275746820626561757479"
+inline_for_extraction
+let size_test1_encryption1_plaintext: size_nat = 29
+let test1_encryption1_plaintext_list : l:list uint8{List.Tot.length l == size_test1_encryption1_plaintext} =
+  [@inline_let]
+  let l = [
+    u8 0x42; u8 0x65; u8 0x61; u8 0x75; u8 0x74;
+    u8 0x79; u8 0x20; u8 0x69; u8 0x73; u8 0x20;
+    u8 0x74; u8 0x72; u8 0x75; u8 0x74; u8 0x68;
+    u8 0x2c; u8 0x20; u8 0x74; u8 0x72; u8 0x75;
+    u8 0x74; u8 0x68; u8 0x20; u8 0x62; u8 0x65;
+    u8 0x61; u8 0x75; u8 0x74; u8 0x79;
+  ] in
+  assert_norm(List.Tot.length l == size_test1_encryption1_plaintext);
+  l
+let test1_encryption1_plaintext : lbytes size_test1_encryption1_plaintext = createL test1_encryption1_plaintext_list
+
+// generated: "436f756e742d32"
+inline_for_extraction
+let size_test1_encryption2_aad: size_nat = 7
+let test1_encryption2_aad_list : l:list uint8{List.Tot.length l == size_test1_encryption2_aad} =
+  [@inline_let]
+  let l = [
+    u8 0x43; u8 0x6f; u8 0x75; u8 0x6e; u8 0x74;
+    u8 0x2d; u8 0x32;
+  ] in
+  assert_norm(List.Tot.length l == size_test1_encryption2_aad);
+  l
+let test1_encryption2_aad : lbytes size_test1_encryption2_aad = createL test1_encryption2_aad_list
+
+// generated: "4bfc8da6f1da808be2c1c141e864fe536bd1e9c4e01376cd383370b8095438a06f372e663739b30af9355da8a3"
+inline_for_extraction
+let size_test1_encryption2_ciphertext: size_nat = 45
+let test1_encryption2_ciphertext_list : l:list uint8{List.Tot.length l == size_test1_encryption2_ciphertext} =
+  [@inline_let]
+  let l = [
+    u8 0x4b; u8 0xfc; u8 0x8d; u8 0xa6; u8 0xf1;
+    u8 0xda; u8 0x80; u8 0x8b; u8 0xe2; u8 0xc1;
+    u8 0xc1; u8 0x41; u8 0xe8; u8 0x64; u8 0xfe;
+    u8 0x53; u8 0x6b; u8 0xd1; u8 0xe9; u8 0xc4;
+    u8 0xe0; u8 0x13; u8 0x76; u8 0xcd; u8 0x38;
+    u8 0x33; u8 0x70; u8 0xb8; u8 0x09; u8 0x54;
+    u8 0x38; u8 0xa0; u8 0x6f; u8 0x37; u8 0x2e;
+    u8 0x66; u8 0x37; u8 0x39; u8 0xb3; u8 0x0a;
+    u8 0xf9; u8 0x35; u8 0x5d; u8 0xa8; u8 0xa3;
+  ] in
+  assert_norm(List.Tot.length l == size_test1_encryption2_ciphertext);
+  l
+let test1_encryption2_ciphertext : lbytes size_test1_encryption2_ciphertext = createL test1_encryption2_ciphertext_list
+
+// generated: "2764228860619e140920c7d5"
+inline_for_extraction
+let size_test1_encryption2_nonce: size_nat = 12
+let test1_encryption2_nonce_list : l:list uint8{List.Tot.length l == size_test1_encryption2_nonce} =
+  [@inline_let]
+  let l = [
+    u8 0x27; u8 0x64; u8 0x22; u8 0x88; u8 0x60;
+    u8 0x61; u8 0x9e; u8 0x14; u8 0x09; u8 0x20;
+    u8 0xc7; u8 0xd5;
+  ] in
+  assert_norm(List.Tot.length l == size_test1_encryption2_nonce);
+  l
+let test1_encryption2_nonce : lbytes size_test1_encryption2_nonce = createL test1_encryption2_nonce_list
+
+// generated: "4265617574792069732074727574682c20747275746820626561757479"
+inline_for_extraction
+let size_test1_encryption2_plaintext: size_nat = 29
+let test1_encryption2_plaintext_list : l:list uint8{List.Tot.length l == size_test1_encryption2_plaintext} =
+  [@inline_let]
+  let l = [
+    u8 0x42; u8 0x65; u8 0x61; u8 0x75; u8 0x74;
+    u8 0x79; u8 0x20; u8 0x69; u8 0x73; u8 0x20;
+    u8 0x74; u8 0x72; u8 0x75; u8 0x74; u8 0x68;
+    u8 0x2c; u8 0x20; u8 0x74; u8 0x72; u8 0x75;
+    u8 0x74; u8 0x68; u8 0x20; u8 0x62; u8 0x65;
+    u8 0x61; u8 0x75; u8 0x74; u8 0x79;
+  ] in
+  assert_norm(List.Tot.length l == size_test1_encryption2_plaintext);
+  l
+let test1_encryption2_plaintext : lbytes size_test1_encryption2_plaintext = createL test1_encryption2_plaintext_list
+
+// generated: "436f756e742d33"
+inline_for_extraction
+let size_test1_encryption3_aad: size_nat = 7
+let test1_encryption3_aad_list : l:list uint8{List.Tot.length l == size_test1_encryption3_aad} =
+  [@inline_let]
+  let l = [
+    u8 0x43; u8 0x6f; u8 0x75; u8 0x6e; u8 0x74;
+    u8 0x2d; u8 0x33;
+  ] in
+  assert_norm(List.Tot.length l == size_test1_encryption3_aad);
+  l
+let test1_encryption3_aad : lbytes size_test1_encryption3_aad = createL test1_encryption3_aad_list
+
+// generated: "cc82487c2beb92d6810a40bad2aa96794c5f2b6eff96a674cf9c9c853397e6c7ca9640c200a38326adb63ed7f2"
+inline_for_extraction
+let size_test1_encryption3_ciphertext: size_nat = 45
+let test1_encryption3_ciphertext_list : l:list uint8{List.Tot.length l == size_test1_encryption3_ciphertext} =
+  [@inline_let]
+  let l = [
+    u8 0xcc; u8 0x82; u8 0x48; u8 0x7c; u8 0x2b;
+    u8 0xeb; u8 0x92; u8 0xd6; u8 0x81; u8 0x0a;
+    u8 0x40; u8 0xba; u8 0xd2; u8 0xaa; u8 0x96;
+    u8 0x79; u8 0x4c; u8 0x5f; u8 0x2b; u8 0x6e;
+    u8 0xff; u8 0x96; u8 0xa6; u8 0x74; u8 0xcf;
+    u8 0x9c; u8 0x9c; u8 0x85; u8 0x33; u8 0x97;
+    u8 0xe6; u8 0xc7; u8 0xca; u8 0x96; u8 0x40;
+    u8 0xc2; u8 0x00; u8 0xa3; u8 0x83; u8 0x26;
+    u8 0xad; u8 0xb6; u8 0x3e; u8 0xd7; u8 0xf2;
+  ] in
+  assert_norm(List.Tot.length l == size_test1_encryption3_ciphertext);
+  l
+let test1_encryption3_ciphertext : lbytes size_test1_encryption3_ciphertext = createL test1_encryption3_ciphertext_list
+
+// generated: "2764228860619e140920c7d4"
+inline_for_extraction
+let size_test1_encryption3_nonce: size_nat = 12
+let test1_encryption3_nonce_list : l:list uint8{List.Tot.length l == size_test1_encryption3_nonce} =
+  [@inline_let]
+  let l = [
+    u8 0x27; u8 0x64; u8 0x22; u8 0x88; u8 0x60;
+    u8 0x61; u8 0x9e; u8 0x14; u8 0x09; u8 0x20;
+    u8 0xc7; u8 0xd4;
+  ] in
+  assert_norm(List.Tot.length l == size_test1_encryption3_nonce);
+  l
+let test1_encryption3_nonce : lbytes size_test1_encryption3_nonce = createL test1_encryption3_nonce_list
+
+// generated: "4265617574792069732074727574682c20747275746820626561757479"
+inline_for_extraction
+let size_test1_encryption3_plaintext: size_nat = 29
+let test1_encryption3_plaintext_list : l:list uint8{List.Tot.length l == size_test1_encryption3_plaintext} =
+  [@inline_let]
+  let l = [
+    u8 0x42; u8 0x65; u8 0x61; u8 0x75; u8 0x74;
+    u8 0x79; u8 0x20; u8 0x69; u8 0x73; u8 0x20;
+    u8 0x74; u8 0x72; u8 0x75; u8 0x74; u8 0x68;
+    u8 0x2c; u8 0x20; u8 0x74; u8 0x72; u8 0x75;
+    u8 0x74; u8 0x68; u8 0x20; u8 0x62; u8 0x65;
+    u8 0x61; u8 0x75; u8 0x74; u8 0x79;
+  ] in
+  assert_norm(List.Tot.length l == size_test1_encryption3_plaintext);
+  l
+let test1_encryption3_plaintext : lbytes size_test1_encryption3_plaintext = createL test1_encryption3_plaintext_list
+
+// generated: "436f756e742d34"
+inline_for_extraction
+let size_test1_encryption4_aad: size_nat = 7
+let test1_encryption4_aad_list : l:list uint8{List.Tot.length l == size_test1_encryption4_aad} =
+  [@inline_let]
+  let l = [
+    u8 0x43; u8 0x6f; u8 0x75; u8 0x6e; u8 0x74;
+    u8 0x2d; u8 0x34;
+  ] in
+  assert_norm(List.Tot.length l == size_test1_encryption4_aad);
+  l
+let test1_encryption4_aad : lbytes size_test1_encryption4_aad = createL test1_encryption4_aad_list
+
+// generated: "6314e60548cfdc30552303be4cb19875e335554bce186e1b41f9d15b4b4a4af77d68c09ebf883a9cbb51f3be9d"
+inline_for_extraction
+let size_test1_encryption4_ciphertext: size_nat = 45
+let test1_encryption4_ciphertext_list : l:list uint8{List.Tot.length l == size_test1_encryption4_ciphertext} =
+  [@inline_let]
+  let l = [
+    u8 0x63; u8 0x14; u8 0xe6; u8 0x05; u8 0x48;
+    u8 0xcf; u8 0xdc; u8 0x30; u8 0x55; u8 0x23;
+    u8 0x03; u8 0xbe; u8 0x4c; u8 0xb1; u8 0x98;
+    u8 0x75; u8 0xe3; u8 0x35; u8 0x55; u8 0x4b;
+    u8 0xce; u8 0x18; u8 0x6e; u8 0x1b; u8 0x41;
+    u8 0xf9; u8 0xd1; u8 0x5b; u8 0x4b; u8 0x4a;
+    u8 0x4a; u8 0xf7; u8 0x7d; u8 0x68; u8 0xc0;
+    u8 0x9e; u8 0xbf; u8 0x88; u8 0x3a; u8 0x9c;
+    u8 0xbb; u8 0x51; u8 0xf3; u8 0xbe; u8 0x9d;
+  ] in
+  assert_norm(List.Tot.length l == size_test1_encryption4_ciphertext);
+  l
+let test1_encryption4_ciphertext : lbytes size_test1_encryption4_ciphertext = createL test1_encryption4_ciphertext_list
+
+// generated: "2764228860619e140920c7d3"
+inline_for_extraction
+let size_test1_encryption4_nonce: size_nat = 12
+let test1_encryption4_nonce_list : l:list uint8{List.Tot.length l == size_test1_encryption4_nonce} =
+  [@inline_let]
+  let l = [
+    u8 0x27; u8 0x64; u8 0x22; u8 0x88; u8 0x60;
+    u8 0x61; u8 0x9e; u8 0x14; u8 0x09; u8 0x20;
+    u8 0xc7; u8 0xd3;
+  ] in
+  assert_norm(List.Tot.length l == size_test1_encryption4_nonce);
+  l
+let test1_encryption4_nonce : lbytes size_test1_encryption4_nonce = createL test1_encryption4_nonce_list
+
+// generated: "4265617574792069732074727574682c20747275746820626561757479"
+inline_for_extraction
+let size_test1_encryption4_plaintext: size_nat = 29
+let test1_encryption4_plaintext_list : l:list uint8{List.Tot.length l == size_test1_encryption4_plaintext} =
+  [@inline_let]
+  let l = [
+    u8 0x42; u8 0x65; u8 0x61; u8 0x75; u8 0x74;
+    u8 0x79; u8 0x20; u8 0x69; u8 0x73; u8 0x20;
+    u8 0x74; u8 0x72; u8 0x75; u8 0x74; u8 0x68;
+    u8 0x2c; u8 0x20; u8 0x74; u8 0x72; u8 0x75;
+    u8 0x74; u8 0x68; u8 0x20; u8 0x62; u8 0x65;
+    u8 0x61; u8 0x75; u8 0x74; u8 0x79;
+  ] in
+  assert_norm(List.Tot.length l == size_test1_encryption4_plaintext);
+  l
+let test1_encryption4_plaintext : lbytes size_test1_encryption4_plaintext = createL test1_encryption4_plaintext_list
+
+// generated: "436f756e742d35"
+inline_for_extraction
+let size_test1_encryption5_aad: size_nat = 7
+let test1_encryption5_aad_list : l:list uint8{List.Tot.length l == size_test1_encryption5_aad} =
+  [@inline_let]
+  let l = [
+    u8 0x43; u8 0x6f; u8 0x75; u8 0x6e; u8 0x74;
+    u8 0x2d; u8 0x35;
+  ] in
+  assert_norm(List.Tot.length l == size_test1_encryption5_aad);
+  l
+let test1_encryption5_aad : lbytes size_test1_encryption5_aad = createL test1_encryption5_aad_list
+
+// generated: "ce580d139c001ed794c4eedf14ce43c19c2a04f20dcfa9de57b6f555816b0558db4ec603bbc3748dce30e5c82f"
+inline_for_extraction
+let size_test1_encryption5_ciphertext: size_nat = 45
+let test1_encryption5_ciphertext_list : l:list uint8{List.Tot.length l == size_test1_encryption5_ciphertext} =
+  [@inline_let]
+  let l = [
+    u8 0xce; u8 0x58; u8 0x0d; u8 0x13; u8 0x9c;
+    u8 0x00; u8 0x1e; u8 0xd7; u8 0x94; u8 0xc4;
+    u8 0xee; u8 0xdf; u8 0x14; u8 0xce; u8 0x43;
+    u8 0xc1; u8 0x9c; u8 0x2a; u8 0x04; u8 0xf2;
+    u8 0x0d; u8 0xcf; u8 0xa9; u8 0xde; u8 0x57;
+    u8 0xb6; u8 0xf5; u8 0x55; u8 0x81; u8 0x6b;
+    u8 0x05; u8 0x58; u8 0xdb; u8 0x4e; u8 0xc6;
+    u8 0x03; u8 0xbb; u8 0xc3; u8 0x74; u8 0x8d;
+    u8 0xce; u8 0x30; u8 0xe5; u8 0xc8; u8 0x2f;
+  ] in
+  assert_norm(List.Tot.length l == size_test1_encryption5_ciphertext);
+  l
+let test1_encryption5_ciphertext : lbytes size_test1_encryption5_ciphertext = createL test1_encryption5_ciphertext_list
+
+// generated: "2764228860619e140920c7d2"
+inline_for_extraction
+let size_test1_encryption5_nonce: size_nat = 12
+let test1_encryption5_nonce_list : l:list uint8{List.Tot.length l == size_test1_encryption5_nonce} =
+  [@inline_let]
+  let l = [
+    u8 0x27; u8 0x64; u8 0x22; u8 0x88; u8 0x60;
+    u8 0x61; u8 0x9e; u8 0x14; u8 0x09; u8 0x20;
+    u8 0xc7; u8 0xd2;
+  ] in
+  assert_norm(List.Tot.length l == size_test1_encryption5_nonce);
+  l
+let test1_encryption5_nonce : lbytes size_test1_encryption5_nonce = createL test1_encryption5_nonce_list
+
+// generated: "4265617574792069732074727574682c20747275746820626561757479"
+inline_for_extraction
+let size_test1_encryption5_plaintext: size_nat = 29
+let test1_encryption5_plaintext_list : l:list uint8{List.Tot.length l == size_test1_encryption5_plaintext} =
+  [@inline_let]
+  let l = [
+    u8 0x42; u8 0x65; u8 0x61; u8 0x75; u8 0x74;
+    u8 0x79; u8 0x20; u8 0x69; u8 0x73; u8 0x20;
+    u8 0x74; u8 0x72; u8 0x75; u8 0x74; u8 0x68;
+    u8 0x2c; u8 0x20; u8 0x74; u8 0x72; u8 0x75;
+    u8 0x74; u8 0x68; u8 0x20; u8 0x62; u8 0x65;
+    u8 0x61; u8 0x75; u8 0x74; u8 0x79;
+  ] in
+  assert_norm(List.Tot.length l == size_test1_encryption5_plaintext);
+  l
+let test1_encryption5_plaintext : lbytes size_test1_encryption5_plaintext = createL test1_encryption5_plaintext_list
+
+// generated: "436f756e742d36"
+inline_for_extraction
+let size_test1_encryption6_aad: size_nat = 7
+let test1_encryption6_aad_list : l:list uint8{List.Tot.length l == size_test1_encryption6_aad} =
+  [@inline_let]
+  let l = [
+    u8 0x43; u8 0x6f; u8 0x75; u8 0x6e; u8 0x74;
+    u8 0x2d; u8 0x36;
+  ] in
+  assert_norm(List.Tot.length l == size_test1_encryption6_aad);
+  l
+let test1_encryption6_aad : lbytes size_test1_encryption6_aad = createL test1_encryption6_aad_list
+
+// generated: "5247db08759b2a6d9459a4cc461dfc59afb78e37b0852f9a669720df72fe5781460bcc9ae5ca00545ad06f93c3"
+inline_for_extraction
+let size_test1_encryption6_ciphertext: size_nat = 45
+let test1_encryption6_ciphertext_list : l:list uint8{List.Tot.length l == size_test1_encryption6_ciphertext} =
+  [@inline_let]
+  let l = [
+    u8 0x52; u8 0x47; u8 0xdb; u8 0x08; u8 0x75;
+    u8 0x9b; u8 0x2a; u8 0x6d; u8 0x94; u8 0x59;
+    u8 0xa4; u8 0xcc; u8 0x46; u8 0x1d; u8 0xfc;
+    u8 0x59; u8 0xaf; u8 0xb7; u8 0x8e; u8 0x37;
+    u8 0xb0; u8 0x85; u8 0x2f; u8 0x9a; u8 0x66;
+    u8 0x97; u8 0x20; u8 0xdf; u8 0x72; u8 0xfe;
+    u8 0x57; u8 0x81; u8 0x46; u8 0x0b; u8 0xcc;
+    u8 0x9a; u8 0xe5; u8 0xca; u8 0x00; u8 0x54;
+    u8 0x5a; u8 0xd0; u8 0x6f; u8 0x93; u8 0xc3;
+  ] in
+  assert_norm(List.Tot.length l == size_test1_encryption6_ciphertext);
+  l
+let test1_encryption6_ciphertext : lbytes size_test1_encryption6_ciphertext = createL test1_encryption6_ciphertext_list
+
+// generated: "2764228860619e140920c7d1"
+inline_for_extraction
+let size_test1_encryption6_nonce: size_nat = 12
+let test1_encryption6_nonce_list : l:list uint8{List.Tot.length l == size_test1_encryption6_nonce} =
+  [@inline_let]
+  let l = [
+    u8 0x27; u8 0x64; u8 0x22; u8 0x88; u8 0x60;
+    u8 0x61; u8 0x9e; u8 0x14; u8 0x09; u8 0x20;
+    u8 0xc7; u8 0xd1;
+  ] in
+  assert_norm(List.Tot.length l == size_test1_encryption6_nonce);
+  l
+let test1_encryption6_nonce : lbytes size_test1_encryption6_nonce = createL test1_encryption6_nonce_list
+
+// generated: "4265617574792069732074727574682c20747275746820626561757479"
+inline_for_extraction
+let size_test1_encryption6_plaintext: size_nat = 29
+let test1_encryption6_plaintext_list : l:list uint8{List.Tot.length l == size_test1_encryption6_plaintext} =
+  [@inline_let]
+  let l = [
+    u8 0x42; u8 0x65; u8 0x61; u8 0x75; u8 0x74;
+    u8 0x79; u8 0x20; u8 0x69; u8 0x73; u8 0x20;
+    u8 0x74; u8 0x72; u8 0x75; u8 0x74; u8 0x68;
+    u8 0x2c; u8 0x20; u8 0x74; u8 0x72; u8 0x75;
+    u8 0x74; u8 0x68; u8 0x20; u8 0x62; u8 0x65;
+    u8 0x61; u8 0x75; u8 0x74; u8 0x79;
+  ] in
+  assert_norm(List.Tot.length l == size_test1_encryption6_plaintext);
+  l
+let test1_encryption6_plaintext : lbytes size_test1_encryption6_plaintext = createL test1_encryption6_plaintext_list
+
+// generated: "436f756e742d37"
+inline_for_extraction
+let size_test1_encryption7_aad: size_nat = 7
+let test1_encryption7_aad_list : l:list uint8{List.Tot.length l == size_test1_encryption7_aad} =
+  [@inline_let]
+  let l = [
+    u8 0x43; u8 0x6f; u8 0x75; u8 0x6e; u8 0x74;
+    u8 0x2d; u8 0x37;
+  ] in
+  assert_norm(List.Tot.length l == size_test1_encryption7_aad);
+  l
+let test1_encryption7_aad : lbytes size_test1_encryption7_aad = createL test1_encryption7_aad_list
+
+// generated: "e4ac909e74ca97d420374dba157678aad8f335b5cdaac2ca2e1813f2b3a6c0f6cfbc690dfd9b04a140861b910b"
+inline_for_extraction
+let size_test1_encryption7_ciphertext: size_nat = 45
+let test1_encryption7_ciphertext_list : l:list uint8{List.Tot.length l == size_test1_encryption7_ciphertext} =
+  [@inline_let]
+  let l = [
+    u8 0xe4; u8 0xac; u8 0x90; u8 0x9e; u8 0x74;
+    u8 0xca; u8 0x97; u8 0xd4; u8 0x20; u8 0x37;
+    u8 0x4d; u8 0xba; u8 0x15; u8 0x76; u8 0x78;
+    u8 0xaa; u8 0xd8; u8 0xf3; u8 0x35; u8 0xb5;
+    u8 0xcd; u8 0xaa; u8 0xc2; u8 0xca; u8 0x2e;
+    u8 0x18; u8 0x13; u8 0xf2; u8 0xb3; u8 0xa6;
+    u8 0xc0; u8 0xf6; u8 0xcf; u8 0xbc; u8 0x69;
+    u8 0x0d; u8 0xfd; u8 0x9b; u8 0x04; u8 0xa1;
+    u8 0x40; u8 0x86; u8 0x1b; u8 0x91; u8 0x0b;
+  ] in
+  assert_norm(List.Tot.length l == size_test1_encryption7_ciphertext);
+  l
+let test1_encryption7_ciphertext : lbytes size_test1_encryption7_ciphertext = createL test1_encryption7_ciphertext_list
+
+// generated: "2764228860619e140920c7d0"
+inline_for_extraction
+let size_test1_encryption7_nonce: size_nat = 12
+let test1_encryption7_nonce_list : l:list uint8{List.Tot.length l == size_test1_encryption7_nonce} =
+  [@inline_let]
+  let l = [
+    u8 0x27; u8 0x64; u8 0x22; u8 0x88; u8 0x60;
+    u8 0x61; u8 0x9e; u8 0x14; u8 0x09; u8 0x20;
+    u8 0xc7; u8 0xd0;
+  ] in
+  assert_norm(List.Tot.length l == size_test1_encryption7_nonce);
+  l
+let test1_encryption7_nonce : lbytes size_test1_encryption7_nonce = createL test1_encryption7_nonce_list
+
+// generated: "4265617574792069732074727574682c20747275746820626561757479"
+inline_for_extraction
+let size_test1_encryption7_plaintext: size_nat = 29
+let test1_encryption7_plaintext_list : l:list uint8{List.Tot.length l == size_test1_encryption7_plaintext} =
+  [@inline_let]
+  let l = [
+    u8 0x42; u8 0x65; u8 0x61; u8 0x75; u8 0x74;
+    u8 0x79; u8 0x20; u8 0x69; u8 0x73; u8 0x20;
+    u8 0x74; u8 0x72; u8 0x75; u8 0x74; u8 0x68;
+    u8 0x2c; u8 0x20; u8 0x74; u8 0x72; u8 0x75;
+    u8 0x74; u8 0x68; u8 0x20; u8 0x62; u8 0x65;
+    u8 0x61; u8 0x75; u8 0x74; u8 0x79;
+  ] in
+  assert_norm(List.Tot.length l == size_test1_encryption7_plaintext);
+  l
+let test1_encryption7_plaintext : lbytes size_test1_encryption7_plaintext = createL test1_encryption7_plaintext_list
+
+// generated: "436f756e742d38"
+inline_for_extraction
+let size_test1_encryption8_aad: size_nat = 7
+let test1_encryption8_aad_list : l:list uint8{List.Tot.length l == size_test1_encryption8_aad} =
+  [@inline_let]
+  let l = [
+    u8 0x43; u8 0x6f; u8 0x75; u8 0x6e; u8 0x74;
+    u8 0x2d; u8 0x38;
+  ] in
+  assert_norm(List.Tot.length l == size_test1_encryption8_aad);
+  l
+let test1_encryption8_aad : lbytes size_test1_encryption8_aad = createL test1_encryption8_aad_list
+
+// generated: "bd664ef7fa8fd4ba23430453914ffa75c54c24a593d894ad6626635ef38792cf505b7925d2f8dcdc744b8a8acd"
+inline_for_extraction
+let size_test1_encryption8_ciphertext: size_nat = 45
+let test1_encryption8_ciphertext_list : l:list uint8{List.Tot.length l == size_test1_encryption8_ciphertext} =
+  [@inline_let]
+  let l = [
+    u8 0xbd; u8 0x66; u8 0x4e; u8 0xf7; u8 0xfa;
+    u8 0x8f; u8 0xd4; u8 0xba; u8 0x23; u8 0x43;
+    u8 0x04; u8 0x53; u8 0x91; u8 0x4f; u8 0xfa;
+    u8 0x75; u8 0xc5; u8 0x4c; u8 0x24; u8 0xa5;
+    u8 0x93; u8 0xd8; u8 0x94; u8 0xad; u8 0x66;
+    u8 0x26; u8 0x63; u8 0x5e; u8 0xf3; u8 0x87;
+    u8 0x92; u8 0xcf; u8 0x50; u8 0x5b; u8 0x79;
+    u8 0x25; u8 0xd2; u8 0xf8; u8 0xdc; u8 0xdc;
+    u8 0x74; u8 0x4b; u8 0x8a; u8 0x8a; u8 0xcd;
+  ] in
+  assert_norm(List.Tot.length l == size_test1_encryption8_ciphertext);
+  l
+let test1_encryption8_ciphertext : lbytes size_test1_encryption8_ciphertext = createL test1_encryption8_ciphertext_list
+
+// generated: "2764228860619e140920c7df"
+inline_for_extraction
+let size_test1_encryption8_nonce: size_nat = 12
+let test1_encryption8_nonce_list : l:list uint8{List.Tot.length l == size_test1_encryption8_nonce} =
+  [@inline_let]
+  let l = [
+    u8 0x27; u8 0x64; u8 0x22; u8 0x88; u8 0x60;
+    u8 0x61; u8 0x9e; u8 0x14; u8 0x09; u8 0x20;
+    u8 0xc7; u8 0xdf;
+  ] in
+  assert_norm(List.Tot.length l == size_test1_encryption8_nonce);
+  l
+let test1_encryption8_nonce : lbytes size_test1_encryption8_nonce = createL test1_encryption8_nonce_list
+
+// generated: "4265617574792069732074727574682c20747275746820626561757479"
+inline_for_extraction
+let size_test1_encryption8_plaintext: size_nat = 29
+let test1_encryption8_plaintext_list : l:list uint8{List.Tot.length l == size_test1_encryption8_plaintext} =
+  [@inline_let]
+  let l = [
+    u8 0x42; u8 0x65; u8 0x61; u8 0x75; u8 0x74;
+    u8 0x79; u8 0x20; u8 0x69; u8 0x73; u8 0x20;
+    u8 0x74; u8 0x72; u8 0x75; u8 0x74; u8 0x68;
+    u8 0x2c; u8 0x20; u8 0x74; u8 0x72; u8 0x75;
+    u8 0x74; u8 0x68; u8 0x20; u8 0x62; u8 0x65;
+    u8 0x61; u8 0x75; u8 0x74; u8 0x79;
+  ] in
+  assert_norm(List.Tot.length l == size_test1_encryption8_plaintext);
+  l
+let test1_encryption8_plaintext : lbytes size_test1_encryption8_plaintext = createL test1_encryption8_plaintext_list
+
+// generated: "436f756e742d39"
+inline_for_extraction
+let size_test1_encryption9_aad: size_nat = 7
+let test1_encryption9_aad_list : l:list uint8{List.Tot.length l == size_test1_encryption9_aad} =
+  [@inline_let]
+  let l = [
+    u8 0x43; u8 0x6f; u8 0x75; u8 0x6e; u8 0x74;
+    u8 0x2d; u8 0x39;
+  ] in
+  assert_norm(List.Tot.length l == size_test1_encryption9_aad);
+  l
+let test1_encryption9_aad : lbytes size_test1_encryption9_aad = createL test1_encryption9_aad_list
+
+// generated: "4b7f4832efecd0a808a367e4d2ac970d6604026e4386211c22912567a061a2558de77f7cb760f1837f6d048d71"
+inline_for_extraction
+let size_test1_encryption9_ciphertext: size_nat = 45
+let test1_encryption9_ciphertext_list : l:list uint8{List.Tot.length l == size_test1_encryption9_ciphertext} =
+  [@inline_let]
+  let l = [
+    u8 0x4b; u8 0x7f; u8 0x48; u8 0x32; u8 0xef;
+    u8 0xec; u8 0xd0; u8 0xa8; u8 0x08; u8 0xa3;
+    u8 0x67; u8 0xe4; u8 0xd2; u8 0xac; u8 0x97;
+    u8 0x0d; u8 0x66; u8 0x04; u8 0x02; u8 0x6e;
+    u8 0x43; u8 0x86; u8 0x21; u8 0x1c; u8 0x22;
+    u8 0x91; u8 0x25; u8 0x67; u8 0xa0; u8 0x61;
+    u8 0xa2; u8 0x55; u8 0x8d; u8 0xe7; u8 0x7f;
+    u8 0x7c; u8 0xb7; u8 0x60; u8 0xf1; u8 0x83;
+    u8 0x7f; u8 0x6d; u8 0x04; u8 0x8d; u8 0x71;
+  ] in
+  assert_norm(List.Tot.length l == size_test1_encryption9_ciphertext);
+  l
+let test1_encryption9_ciphertext : lbytes size_test1_encryption9_ciphertext = createL test1_encryption9_ciphertext_list
+
+// generated: "2764228860619e140920c7de"
+inline_for_extraction
+let size_test1_encryption9_nonce: size_nat = 12
+let test1_encryption9_nonce_list : l:list uint8{List.Tot.length l == size_test1_encryption9_nonce} =
+  [@inline_let]
+  let l = [
+    u8 0x27; u8 0x64; u8 0x22; u8 0x88; u8 0x60;
+    u8 0x61; u8 0x9e; u8 0x14; u8 0x09; u8 0x20;
+    u8 0xc7; u8 0xde;
+  ] in
+  assert_norm(List.Tot.length l == size_test1_encryption9_nonce);
+  l
+let test1_encryption9_nonce : lbytes size_test1_encryption9_nonce = createL test1_encryption9_nonce_list
+
+// generated: "4265617574792069732074727574682c20747275746820626561757479"
+inline_for_extraction
+let size_test1_encryption9_plaintext: size_nat = 29
+let test1_encryption9_plaintext_list : l:list uint8{List.Tot.length l == size_test1_encryption9_plaintext} =
+  [@inline_let]
+  let l = [
+    u8 0x42; u8 0x65; u8 0x61; u8 0x75; u8 0x74;
+    u8 0x79; u8 0x20; u8 0x69; u8 0x73; u8 0x20;
+    u8 0x74; u8 0x72; u8 0x75; u8 0x74; u8 0x68;
+    u8 0x2c; u8 0x20; u8 0x74; u8 0x72; u8 0x75;
+    u8 0x74; u8 0x68; u8 0x20; u8 0x62; u8 0x65;
+    u8 0x61; u8 0x75; u8 0x74; u8 0x79;
+  ] in
+  assert_norm(List.Tot.length l == size_test1_encryption9_plaintext);
+  l
+let test1_encryption9_plaintext : lbytes size_test1_encryption9_plaintext = createL test1_encryption9_plaintext_list
+
+// generated: "436f6e746578742d30"
+inline_for_extraction
+let size_test1_export0_exportContext: size_nat = 9
+let test1_export0_exportContext_list : l:list uint8{List.Tot.length l == size_test1_export0_exportContext} =
+  [@inline_let]
+  let l = [
+    u8 0x43; u8 0x6f; u8 0x6e; u8 0x74; u8 0x65;
+    u8 0x78; u8 0x74; u8 0x2d; u8 0x30;
+  ] in
+  assert_norm(List.Tot.length l == size_test1_export0_exportContext);
+  l
+let test1_export0_exportContext : lbytes size_test1_export0_exportContext = createL test1_export0_exportContext_list
+
+// generated: "76d8f9425846916bf678504e398e984d91878220f34c5a5e1a63ac75ba0176bc"
+inline_for_extraction
+let size_test1_export0_exportValue: size_nat = 32
+let test1_export0_exportValue_list : l:list uint8{List.Tot.length l == size_test1_export0_exportValue} =
+  [@inline_let]
+  let l = [
+    u8 0x76; u8 0xd8; u8 0xf9; u8 0x42; u8 0x58;
+    u8 0x46; u8 0x91; u8 0x6b; u8 0xf6; u8 0x78;
+    u8 0x50; u8 0x4e; u8 0x39; u8 0x8e; u8 0x98;
+    u8 0x4d; u8 0x91; u8 0x87; u8 0x82; u8 0x20;
+    u8 0xf3; u8 0x4c; u8 0x5a; u8 0x5e; u8 0x1a;
+    u8 0x63; u8 0xac; u8 0x75; u8 0xba; u8 0x01;
+    u8 0x76; u8 0xbc;
+  ] in
+  assert_norm(List.Tot.length l == size_test1_export0_exportValue);
+  l
+let test1_export0_exportValue : lbytes size_test1_export0_exportValue = createL test1_export0_exportValue_list
+
+let test1_export0_len:size_nat = 32
+// generated: "436f6e746578742d31"
+inline_for_extraction
+let size_test1_export1_exportContext: size_nat = 9
+let test1_export1_exportContext_list : l:list uint8{List.Tot.length l == size_test1_export1_exportContext} =
+  [@inline_let]
+  let l = [
+    u8 0x43; u8 0x6f; u8 0x6e; u8 0x74; u8 0x65;
+    u8 0x78; u8 0x74; u8 0x2d; u8 0x31;
+  ] in
+  assert_norm(List.Tot.length l == size_test1_export1_exportContext);
+  l
+let test1_export1_exportContext : lbytes size_test1_export1_exportContext = createL test1_export1_exportContext_list
+
+// generated: "94fe3245047dde534862778ca1962e594b1758df5a525b4caa54ff0feadad06b"
+inline_for_extraction
+let size_test1_export1_exportValue: size_nat = 32
+let test1_export1_exportValue_list : l:list uint8{List.Tot.length l == size_test1_export1_exportValue} =
+  [@inline_let]
+  let l = [
+    u8 0x94; u8 0xfe; u8 0x32; u8 0x45; u8 0x04;
+    u8 0x7d; u8 0xde; u8 0x53; u8 0x48; u8 0x62;
+    u8 0x77; u8 0x8c; u8 0xa1; u8 0x96; u8 0x2e;
+    u8 0x59; u8 0x4b; u8 0x17; u8 0x58; u8 0xdf;
+    u8 0x5a; u8 0x52; u8 0x5b; u8 0x4c; u8 0xaa;
+    u8 0x54; u8 0xff; u8 0x0f; u8 0xea; u8 0xda;
+    u8 0xd0; u8 0x6b;
+  ] in
+  assert_norm(List.Tot.length l == size_test1_export1_exportValue);
+  l
+let test1_export1_exportValue : lbytes size_test1_export1_exportValue = createL test1_export1_exportValue_list
+
+let test1_export1_len:size_nat = 32
+// generated: "436f6e746578742d32"
+inline_for_extraction
+let size_test1_export2_exportContext: size_nat = 9
+let test1_export2_exportContext_list : l:list uint8{List.Tot.length l == size_test1_export2_exportContext} =
+  [@inline_let]
+  let l = [
+    u8 0x43; u8 0x6f; u8 0x6e; u8 0x74; u8 0x65;
+    u8 0x78; u8 0x74; u8 0x2d; u8 0x32;
+  ] in
+  assert_norm(List.Tot.length l == size_test1_export2_exportContext);
+  l
+let test1_export2_exportContext : lbytes size_test1_export2_exportContext = createL test1_export2_exportContext_list
+
+// generated: "97f0c64128ff1379af9ec623cba204b50cd9db9a6b7d90e7a28fed06badf363e"
+inline_for_extraction
+let size_test1_export2_exportValue: size_nat = 32
+let test1_export2_exportValue_list : l:list uint8{List.Tot.length l == size_test1_export2_exportValue} =
+  [@inline_let]
+  let l = [
+    u8 0x97; u8 0xf0; u8 0xc6; u8 0x41; u8 0x28;
+    u8 0xff; u8 0x13; u8 0x79; u8 0xaf; u8 0x9e;
+    u8 0xc6; u8 0x23; u8 0xcb; u8 0xa2; u8 0x04;
+    u8 0xb5; u8 0x0c; u8 0xd9; u8 0xdb; u8 0x9a;
+    u8 0x6b; u8 0x7d; u8 0x90; u8 0xe7; u8 0xa2;
+    u8 0x8f; u8 0xed; u8 0x06; u8 0xba; u8 0xdf;
+    u8 0x36; u8 0x3e;
+  ] in
+  assert_norm(List.Tot.length l == size_test1_export2_exportValue);
+  l
+let test1_export2_exportValue : lbytes size_test1_export2_exportValue = createL test1_export2_exportValue_list
+
+let test1_export2_len:size_nat = 32
+// generated: "436f6e746578742d33"
+inline_for_extraction
+let size_test1_export3_exportContext: size_nat = 9
+let test1_export3_exportContext_list : l:list uint8{List.Tot.length l == size_test1_export3_exportContext} =
+  [@inline_let]
+  let l = [
+    u8 0x43; u8 0x6f; u8 0x6e; u8 0x74; u8 0x65;
+    u8 0x78; u8 0x74; u8 0x2d; u8 0x33;
+  ] in
+  assert_norm(List.Tot.length l == size_test1_export3_exportContext);
+  l
+let test1_export3_exportContext : lbytes size_test1_export3_exportContext = createL test1_export3_exportContext_list
+
+// generated: "9cd27f832e7271f82ae85c3404d7d06ab2a5bebb9354bc022b9f016d74bcdb2c"
+inline_for_extraction
+let size_test1_export3_exportValue: size_nat = 32
+let test1_export3_exportValue_list : l:list uint8{List.Tot.length l == size_test1_export3_exportValue} =
+  [@inline_let]
+  let l = [
+    u8 0x9c; u8 0xd2; u8 0x7f; u8 0x83; u8 0x2e;
+    u8 0x72; u8 0x71; u8 0xf8; u8 0x2a; u8 0xe8;
+    u8 0x5c; u8 0x34; u8 0x04; u8 0xd7; u8 0xd0;
+    u8 0x6a; u8 0xb2; u8 0xa5; u8 0xbe; u8 0xbb;
+    u8 0x93; u8 0x54; u8 0xbc; u8 0x02; u8 0x2b;
+    u8 0x9f; u8 0x01; u8 0x6d; u8 0x74; u8 0xbc;
+    u8 0xdb; u8 0x2c;
+  ] in
+  assert_norm(List.Tot.length l == size_test1_export3_exportValue);
+  l
+let test1_export3_exportValue : lbytes size_test1_export3_exportValue = createL test1_export3_exportValue_list
+
+let test1_export3_len:size_nat = 32
+// generated: "436f6e746578742d34"
+inline_for_extraction
+let size_test1_export4_exportContext: size_nat = 9
+let test1_export4_exportContext_list : l:list uint8{List.Tot.length l == size_test1_export4_exportContext} =
+  [@inline_let]
+  let l = [
+    u8 0x43; u8 0x6f; u8 0x6e; u8 0x74; u8 0x65;
+    u8 0x78; u8 0x74; u8 0x2d; u8 0x34;
+  ] in
+  assert_norm(List.Tot.length l == size_test1_export4_exportContext);
+  l
+let test1_export4_exportContext : lbytes size_test1_export4_exportContext = createL test1_export4_exportContext_list
+
+// generated: "74da0b06441dd2aca2a43d5ee4796158c9403f7037e93c50bcbd6ea4a1687c06"
+inline_for_extraction
+let size_test1_export4_exportValue: size_nat = 32
+let test1_export4_exportValue_list : l:list uint8{List.Tot.length l == size_test1_export4_exportValue} =
+  [@inline_let]
+  let l = [
+    u8 0x74; u8 0xda; u8 0x0b; u8 0x06; u8 0x44;
+    u8 0x1d; u8 0xd2; u8 0xac; u8 0xa2; u8 0xa4;
+    u8 0x3d; u8 0x5e; u8 0xe4; u8 0x79; u8 0x61;
+    u8 0x58; u8 0xc9; u8 0x40; u8 0x3f; u8 0x70;
+    u8 0x37; u8 0xe9; u8 0x3c; u8 0x50; u8 0xbc;
+    u8 0xbd; u8 0x6e; u8 0xa4; u8 0xa1; u8 0x68;
+    u8 0x7c; u8 0x06;
+  ] in
+  assert_norm(List.Tot.length l == size_test1_export4_exportValue);
+  l
+let test1_export4_exportValue : lbytes size_test1_export4_exportValue = createL test1_export4_exportValue_list
+
+let test1_export4_len:size_nat = 32
 
 
-let test1_pskID = List.Tot.map u8_from_UInt8 [
-  0x45uy; 0x6euy; 0x6euy; 0x79uy; 0x6euy;
-  0x20uy; 0x44uy; 0x75uy; 0x72uy; 0x69uy;
-  0x6euy; 0x20uy; 0x61uy; 0x72uy; 0x61uy;
-  0x6euy; 0x20uy; 0x4duy; 0x6fuy; 0x72uy;
-  0x69uy; 0x61uy
-]
+(* let test1_mode: HPKE.mode = HPKE.Base *)
+(* let test1_ciphersuite = DH.DH_Curve25519, Hash.SHA2_256, AEAD.AES128_GCM, Hash.SHA2_256 *)
+(* // generated: "4f6465206f6e2061204772656369616e2055726e" *)
+(* let test1_info = List.Tot.map u8_from_UInt8 [ *)
+(*   0x4fuy; 0x64uy; 0x65uy; 0x20uy; 0x6fuy; *)
+(*   0x6euy; 0x20uy; 0x61uy; 0x20uy; 0x47uy; *)
+(*   0x72uy; 0x65uy; 0x63uy; 0x69uy; 0x61uy; *)
+(*   0x6euy; 0x20uy; 0x55uy; 0x72uy; 0x6euy; *)
+(* ] *)
 
-let test1_pkR = List.Tot.map u8_from_UInt8 [
-  0x14uy; 0xfduy; 0xb8uy; 0x07uy; 0xc7uy;
-  0x9fuy; 0xb7uy; 0x87uy; 0xd4uy; 0x78uy;
-  0x90uy; 0xd5uy; 0x02uy; 0xbcuy; 0xe7uy;
-  0xc3uy; 0x35uy; 0xd0uy; 0x80uy; 0x9auy;
-  0x05uy; 0x3buy; 0x92uy; 0x87uy; 0xe3uy;
-  0x0fuy; 0xc6uy; 0x08uy; 0xfcuy; 0xfcuy;
-  0x9duy; 0x26uy;
-]
+(* // generated: "919f0e1b7c361d1e5a3d0086ba94edeb6d2df9f756654741731f4e84cb813bdb" *)
+(* let test1_skRm = List.Tot.map u8_from_UInt8 [ *)
+(*   0x91uy; 0x9fuy; 0x0euy; 0x1buy; 0x7cuy; *)
+(*   0x36uy; 0x1duy; 0x1euy; 0x5auy; 0x3duy; *)
+(*   0x00uy; 0x86uy; 0xbauy; 0x94uy; 0xeduy; *)
+(*   0xebuy; 0x6duy; 0x2duy; 0xf9uy; 0xf7uy; *)
+(*   0x56uy; 0x65uy; 0x47uy; 0x41uy; 0x73uy; *)
+(*   0x1fuy; 0x4euy; 0x84uy; 0xcbuy; 0x81uy; *)
+(*   0x3buy; 0xdbuy; *)
+(* ] *)
 
-let test1_pkI = List.Tot.map u8_from_UInt8 [
-  0x6euy; 0xacuy; 0x89uy; 0xbcuy; 0x5duy;
-  0x63uy; 0xe7uy; 0xb4uy; 0x0cuy; 0x39uy;
-  0x4auy; 0x42uy; 0x18uy; 0xb6uy; 0xa8uy;
-  0x20uy; 0x38uy; 0x03uy; 0x74uy; 0x9fuy;
-  0x95uy; 0xfcuy; 0xa2uy; 0x36uy; 0x96uy;
-  0x11uy; 0xeduy; 0x41uy; 0xafuy; 0xb9uy;
-  0x7euy; 0x06uy;
-]
+(* // generated: "232ce0da9fd45b8d500781a5ee1b0a2cf64411dd08d6442400ab05a4d29733a8" *)
+(* let test1_skEm = List.Tot.map u8_from_UInt8 [ *)
+(*   0x23uy; 0x2cuy; 0xe0uy; 0xdauy; 0x9fuy; *)
+(*   0xd4uy; 0x5buy; 0x8duy; 0x50uy; 0x07uy; *)
+(*   0x81uy; 0xa5uy; 0xeeuy; 0x1buy; 0x0auy; *)
+(*   0x2cuy; 0xf6uy; 0x44uy; 0x11uy; 0xdduy; *)
+(*   0x08uy; 0xd6uy; 0x44uy; 0x24uy; 0x00uy; *)
+(*   0xabuy; 0x05uy; 0xa4uy; 0xd2uy; 0x97uy; *)
+(*   0x33uy; 0xa8uy; *)
+(* ] *)
 
-let test1_pkE = List.Tot.map u8_from_UInt8 [
-  0x04uy; 0x54uy; 0xa5uy; 0xa1uy; 0x0euy;
-  0xcauy; 0xf9uy; 0x82uy; 0x21uy; 0x9euy;
-  0xaeuy; 0x4buy; 0x5cuy; 0x36uy; 0xbcuy;
-  0x3euy; 0x16uy; 0x06uy; 0x81uy; 0x3cuy;
-  0xaauy; 0xe1uy; 0xd2uy; 0x62uy; 0x52uy;
-  0x83uy; 0x96uy; 0xc6uy; 0x0duy; 0xe4uy;
-  0x4euy; 0x3duy;
-]
+(* // generated: "ac511615dee12b2e11170f1272c3972e6e2268d8fb05fc93c6b008065f61f22f" *)
+(* let test1_pkRm = List.Tot.map u8_from_UInt8 [ *)
+(*   0xacuy; 0x51uy; 0x16uy; 0x15uy; 0xdeuy; *)
+(*   0xe1uy; 0x2buy; 0x2euy; 0x11uy; 0x17uy; *)
+(*   0x0fuy; 0x12uy; 0x72uy; 0xc3uy; 0x97uy; *)
+(*   0x2euy; 0x6euy; 0x22uy; 0x68uy; 0xd8uy; *)
+(*   0xfbuy; 0x05uy; 0xfcuy; 0x93uy; 0xc6uy; *)
+(*   0xb0uy; 0x08uy; 0x06uy; 0x5fuy; 0x61uy; *)
+(*   0xf2uy; 0x2fuy; *)
+(* ] *)
 
-let test1_enc = List.Tot.map u8_from_UInt8 [
-  0x04uy; 0x54uy; 0xa5uy; 0xa1uy; 0x0euy;
-  0xcauy; 0xf9uy; 0x82uy; 0x21uy; 0x9euy;
-  0xaeuy; 0x4buy; 0x5cuy; 0x36uy; 0xbcuy;
-  0x3euy; 0x16uy; 0x06uy; 0x81uy; 0x3cuy;
-  0xaauy; 0xe1uy; 0xd2uy; 0x62uy; 0x52uy;
-  0x83uy; 0x96uy; 0xc6uy; 0x0duy; 0xe4uy;
-  0x4euy; 0x3duy;
-]
+(* // generated: "ab8b7fdda7ed10c410079909350948ff63bc044b40575cc85636f3981bb8d258" *)
+(* let test1_pkEm = List.Tot.map u8_from_UInt8 [ *)
+(*   0xabuy; 0x8buy; 0x7fuy; 0xdduy; 0xa7uy; *)
+(*   0xeduy; 0x10uy; 0xc4uy; 0x10uy; 0x07uy; *)
+(*   0x99uy; 0x09uy; 0x35uy; 0x09uy; 0x48uy; *)
+(*   0xffuy; 0x63uy; 0xbcuy; 0x04uy; 0x4buy; *)
+(*   0x40uy; 0x57uy; 0x5cuy; 0xc8uy; 0x56uy; *)
+(*   0x36uy; 0xf3uy; 0x98uy; 0x1buy; 0xb8uy; *)
+(*   0xd2uy; 0x58uy; *)
+(* ] *)
 
-let test1_zz = List.Tot.map u8_from_UInt8 [
-  0x15uy; 0x17uy; 0x8euy; 0xf7uy; 0x72uy;
-  0x62uy; 0xb0uy; 0x46uy; 0x8euy; 0xe8uy;
-  0x28uy; 0xa6uy; 0xdauy; 0x4fuy; 0x26uy;
-  0x20uy; 0x43uy; 0x4auy; 0x9euy; 0xdfuy;
-  0xdduy; 0xdfuy; 0xe9uy; 0x25uy; 0x6auy;
-  0xc5uy; 0x3fuy; 0x8cuy; 0x6buy; 0x7euy;
-  0x57uy; 0x5duy;
-]
+(* // generated: "ab8b7fdda7ed10c410079909350948ff63bc044b40575cc85636f3981bb8d258" *)
+(* let test1_enc = List.Tot.map u8_from_UInt8 [ *)
+(*   0xabuy; 0x8buy; 0x7fuy; 0xdduy; 0xa7uy; *)
+(*   0xeduy; 0x10uy; 0xc4uy; 0x10uy; 0x07uy; *)
+(*   0x99uy; 0x09uy; 0x35uy; 0x09uy; 0x48uy; *)
+(*   0xffuy; 0x63uy; 0xbcuy; 0x04uy; 0x4buy; *)
+(*   0x40uy; 0x57uy; 0x5cuy; 0xc8uy; 0x56uy; *)
+(*   0x36uy; 0xf3uy; 0x98uy; 0x1buy; 0xb8uy; *)
+(*   0xd2uy; 0x58uy; *)
+(* ] *)
 
-let test1_context = List.Tot.map u8_from_UInt8 [
-  0x00uy; 0x00uy; 0x02uy; 0x00uy; 0x01uy;
-  0x00uy; 0x01uy; 0x04uy; 0x54uy; 0xa5uy;
-  0xa1uy; 0x0euy; 0xcauy; 0xf9uy; 0x82uy;
-  0x21uy; 0x9euy; 0xaeuy; 0x4buy; 0x5cuy;
-  0x36uy; 0xbcuy; 0x3euy; 0x16uy; 0x06uy;
-  0x81uy; 0x3cuy; 0xaauy; 0xe1uy; 0xd2uy;
-  0x62uy; 0x52uy; 0x83uy; 0x96uy; 0xc6uy;
-  0x0duy; 0xe4uy; 0x4euy; 0x3duy; 0x14uy;
-  0xfduy; 0xb8uy; 0x07uy; 0xc7uy; 0x9fuy;
-  0xb7uy; 0x87uy; 0xd4uy; 0x78uy; 0x90uy;
-  0xd5uy; 0x02uy; 0xbcuy; 0xe7uy; 0xc3uy;
-  0x35uy; 0xd0uy; 0x80uy; 0x9auy; 0x05uy;
-  0x3buy; 0x92uy; 0x87uy; 0xe3uy; 0x0fuy;
-  0xc6uy; 0x08uy; 0xfcuy; 0xfcuy; 0x9duy;
-  0x26uy; 0x00uy; 0x00uy; 0x00uy; 0x00uy;
-  0x00uy; 0x00uy; 0x00uy; 0x00uy; 0x00uy;
-  0x00uy; 0x00uy; 0x00uy; 0x00uy; 0x00uy;
-  0x00uy; 0x00uy; 0x00uy; 0x00uy; 0x00uy;
-  0x00uy; 0x00uy; 0x00uy; 0x00uy; 0x00uy;
-  0x00uy; 0x00uy; 0x00uy; 0x00uy; 0x00uy;
-  0x00uy; 0x00uy; 0x00uy; 0xe3uy; 0xb0uy;
-  0xc4uy; 0x42uy; 0x98uy; 0xfcuy; 0x1cuy;
-  0x14uy; 0x9auy; 0xfbuy; 0xf4uy; 0xc8uy;
-  0x99uy; 0x6fuy; 0xb9uy; 0x24uy; 0x27uy;
-  0xaeuy; 0x41uy; 0xe4uy; 0x64uy; 0x9buy;
-  0x93uy; 0x4cuy; 0xa4uy; 0x95uy; 0x99uy;
-  0x1buy; 0x78uy; 0x52uy; 0xb8uy; 0x55uy;
-  0x55uy; 0xc4uy; 0x04uy; 0x06uy; 0x29uy;
-  0xc6uy; 0x4cuy; 0x5euy; 0xfeuy; 0xc2uy;
-  0xf7uy; 0x23uy; 0x04uy; 0x07uy; 0xd6uy;
-  0x12uy; 0xd1uy; 0x62uy; 0x89uy; 0xd7uy;
-  0xc5uy; 0xd7uy; 0xafuy; 0xcfuy; 0x93uy;
-  0x40uy; 0x28uy; 0x0auy; 0xbduy; 0x2duy;
-  0xe1uy; 0xabuy;
-]
+(* // generated: "44807c99177b0f3761d66f422945a21317a1532ca038e976594487a6a7e58fbf" *)
+(* let test1_zz = List.Tot.map u8_from_UInt8 [ *)
+(*   0x44uy; 0x80uy; 0x7cuy; 0x99uy; 0x17uy; *)
+(*   0x7buy; 0x0fuy; 0x37uy; 0x61uy; 0xd6uy; *)
+(*   0x6fuy; 0x42uy; 0x29uy; 0x45uy; 0xa2uy; *)
+(*   0x13uy; 0x17uy; 0xa1uy; 0x53uy; 0x2cuy; *)
+(*   0xa0uy; 0x38uy; 0xe9uy; 0x76uy; 0x59uy; *)
+(*   0x44uy; 0x87uy; 0xa6uy; 0xa7uy; 0xe5uy; *)
+(*   0x8fuy; 0xbfuy; *)
+(* ] *)
 
-let test1_secret = List.Tot.map u8_from_UInt8 [
-  0xc5uy; 0xfduy; 0xbbuy; 0xaduy; 0x5cuy;
-  0x72uy; 0xeduy; 0x70uy; 0x35uy; 0x81uy;
-  0xbbuy; 0xcduy; 0x3fuy; 0xe8uy; 0x90uy;
-  0xa7uy; 0xeduy; 0x46uy; 0xd6uy; 0xbfuy;
-  0x00uy; 0xc7uy; 0x3cuy; 0x97uy; 0x55uy;
-  0xbfuy; 0xfbuy; 0xcduy; 0x67uy; 0x44uy;
-  0xf2uy; 0x2buy;
-]
+(* // generated: "002000010001005d0f5548cb13d7eba5320ae0e21b1ee274aac7ea1cce02570cf993d1b2456449debcca602075cf6f8ef506613a82e1c73727e2c912d0c49f16cd56fc524af4ce" *)
+(* let test1_key_schedule_context = List.Tot.map u8_from_UInt8 [ *)
+(*   0x00uy; 0x20uy; 0x00uy; 0x01uy; 0x00uy; *)
+(*   0x01uy; 0x00uy; 0x5duy; 0x0fuy; 0x55uy; *)
+(*   0x48uy; 0xcbuy; 0x13uy; 0xd7uy; 0xebuy; *)
+(*   0xa5uy; 0x32uy; 0x0auy; 0xe0uy; 0xe2uy; *)
+(*   0x1buy; 0x1euy; 0xe2uy; 0x74uy; 0xaauy; *)
+(*   0xc7uy; 0xeauy; 0x1cuy; 0xceuy; 0x02uy; *)
+(*   0x57uy; 0x0cuy; 0xf9uy; 0x93uy; 0xd1uy; *)
+(*   0xb2uy; 0x45uy; 0x64uy; 0x49uy; 0xdeuy; *)
+(*   0xbcuy; 0xcauy; 0x60uy; 0x20uy; 0x75uy; *)
+(*   0xcfuy; 0x6fuy; 0x8euy; 0xf5uy; 0x06uy; *)
+(*   0x61uy; 0x3auy; 0x82uy; 0xe1uy; 0xc7uy; *)
+(*   0x37uy; 0x27uy; 0xe2uy; 0xc9uy; 0x12uy; *)
+(*   0xd0uy; 0xc4uy; 0x9fuy; 0x16uy; 0xcduy; *)
+(*   0x56uy; 0xfcuy; 0x52uy; 0x4auy; 0xf4uy; *)
+(*   0xceuy; *)
+(* ] *)
 
-let test1_key = List.Tot.map u8_from_UInt8 [
-  0x11uy; 0xcfuy; 0x34uy; 0xf9uy; 0x3buy;
-  0x3duy; 0x1euy; 0x8fuy; 0x2euy; 0x36uy;
-  0xf9uy; 0x1cuy; 0x5auy; 0x2duy; 0x68uy;
-  0x18uy;
-]
+(* // generated: "c104521df56de97b517165011f09e0ea2a36b9af339a9de402c8b88547c8b67e" *)
+(* let test1_secret = List.Tot.map u8_from_UInt8 [ *)
+(*   0xc1uy; 0x04uy; 0x52uy; 0x1duy; 0xf5uy; *)
+(*   0x6duy; 0xe9uy; 0x7buy; 0x51uy; 0x71uy; *)
+(*   0x65uy; 0x01uy; 0x1fuy; 0x09uy; 0xe0uy; *)
+(*   0xeauy; 0x2auy; 0x36uy; 0xb9uy; 0xafuy; *)
+(*   0x33uy; 0x9auy; 0x9duy; 0xe4uy; 0x02uy; *)
+(*   0xc8uy; 0xb8uy; 0x85uy; 0x47uy; 0xc8uy; *)
+(*   0xb6uy; 0x7euy; *)
+(* ] *)
 
-let test1_nonce = List.Tot.map u8_from_UInt8 [
-  0x23uy; 0xacuy; 0xefuy; 0x66uy; 0x9duy;
-  0x7fuy; 0x3buy; 0xccuy; 0x98uy; 0xf6uy;
-  0xd0uy; 0xabuy;
-]
+(* // generated: "e34afc8f8f4c2906b310d8e4e4d526f0" *)
+(* let test1_key = List.Tot.map u8_from_UInt8 [ *)
+(*   0xe3uy; 0x4auy; 0xfcuy; 0x8fuy; 0x8fuy; *)
+(*   0x4cuy; 0x29uy; 0x06uy; 0xb3uy; 0x10uy; *)
+(*   0xd8uy; 0xe4uy; 0xe4uy; 0xd5uy; 0x26uy; *)
+(*   0xf0uy; *)
+(* ] *)
 
-let test1_plaintext = List.Tot.map u8_from_UInt8 [
-  0x42uy; 0x65uy; 0x61uy; 0x75uy; 0x74uy;
-  0x79uy; 0x20uy; 0x69uy; 0x73uy; 0x20uy;
-  0x74uy; 0x72uy; 0x75uy; 0x74uy; 0x68uy;
-  0x2cuy; 0x20uy; 0x74uy; 0x72uy; 0x75uy;
-  0x74uy; 0x68uy; 0x20uy; 0x62uy; 0x65uy;
-  0x61uy; 0x75uy; 0x74uy; 0x79uy;
-]
+(* // generated: "2764228860619e140920c7d7" *)
+(* let test1_nonce = List.Tot.map u8_from_UInt8 [ *)
+(*   0x27uy; 0x64uy; 0x22uy; 0x88uy; 0x60uy; *)
+(*   0x61uy; 0x9euy; 0x14uy; 0x09uy; 0x20uy; *)
+(*   0xc7uy; 0xd7uy; *)
+(* ] *)
 
-let test1_aad0 = List.Tot.map u8_from_UInt8 [
-  0x43uy; 0x6fuy; 0x75uy; 0x6euy; 0x74uy;
-  0x2duy; 0x30uy;
-]
+(* // generated: "93c6a28ec7af55f669612d5d64fe680ae38ca88d14fb6ecba647606eee668124" *)
+(* let test1_exporterSecret = List.Tot.map u8_from_UInt8 [ *)
+(*   0x93uy; 0xc6uy; 0xa2uy; 0x8euy; 0xc7uy; *)
+(*   0xafuy; 0x55uy; 0xf6uy; 0x69uy; 0x61uy; *)
+(*   0x2duy; 0x5duy; 0x64uy; 0xfeuy; 0x68uy; *)
+(*   0x0auy; 0xe3uy; 0x8cuy; 0xa8uy; 0x8duy; *)
+(*   0x14uy; 0xfbuy; 0x6euy; 0xcbuy; 0xa6uy; *)
+(*   0x47uy; 0x60uy; 0x6euy; 0xeeuy; 0x66uy; *)
+(*   0x81uy; 0x24uy; *)
+(* ] *)
 
-let test1_nonce0 = List.Tot.map u8_from_UInt8 [
-  0x23uy; 0xacuy; 0xefuy; 0x66uy; 0x9duy;
-  0x7fuy; 0x3buy; 0xccuy; 0x98uy; 0xf6uy;
-  0xd0uy; 0xabuy;
-]
+(* // generated: "436f756e742d30" *)
+(* let test1_encryption0_aad = List.Tot.map u8_from_UInt8 [ *)
+(*   0x43uy; 0x6fuy; 0x75uy; 0x6euy; 0x74uy; *)
+(*   0x2duy; 0x30uy; *)
+(* ] *)
 
-let test1_cipher0 = List.Tot.map u8_from_UInt8 [
-  0x13uy; 0xfcuy; 0x68uy; 0xaeuy; 0xf8uy;
-  0xe2uy; 0xc4uy; 0x59uy; 0x1auy; 0x0duy;
-  0xd9uy; 0x2cuy; 0x01uy; 0xffuy; 0xe9uy;
-  0x57uy; 0x33uy; 0x14uy; 0xd8uy; 0x81uy;
-  0xcfuy; 0x71uy; 0xdduy; 0x57uy; 0x08uy;
-  0x64uy; 0x4euy; 0xe7uy; 0x18uy; 0x48uy;
-  0x18uy; 0xe4uy; 0x57uy; 0xdeuy; 0x3buy;
-  0x4duy; 0x51uy; 0xebuy; 0x1duy; 0xebuy;
-  0x4fuy; 0x0buy; 0xebuy; 0x35uy; 0xd1uy;
-]
+(* // generated: "1811cf5d39f857f80175f96ca4d3600bfb0585e4ce119bc46396da4b371966a358924e5a97a7b53ea255971f6b" *)
+(* let test1_encryption0_ciphertext = List.Tot.map u8_from_UInt8 [ *)
+(*   0x18uy; 0x11uy; 0xcfuy; 0x5duy; 0x39uy; *)
+(*   0xf8uy; 0x57uy; 0xf8uy; 0x01uy; 0x75uy; *)
+(*   0xf9uy; 0x6cuy; 0xa4uy; 0xd3uy; 0x60uy; *)
+(*   0x0buy; 0xfbuy; 0x05uy; 0x85uy; 0xe4uy; *)
+(*   0xceuy; 0x11uy; 0x9buy; 0xc4uy; 0x63uy; *)
+(*   0x96uy; 0xdauy; 0x4buy; 0x37uy; 0x19uy; *)
+(*   0x66uy; 0xa3uy; 0x58uy; 0x92uy; 0x4euy; *)
+(*   0x5auy; 0x97uy; 0xa7uy; 0xb5uy; 0x3euy; *)
+(*   0xa2uy; 0x55uy; 0x97uy; 0x1fuy; 0x6buy; *)
+(* ] *)
 
-// DHKEM(P-256), HKDF-SHA256, ChaCha20Poly1305
-// Base Setup
-// mode: 0
-// kemID: 1
-// kdfID: 1
-// aeadID: 3
-// info: 4f6465206f6e2061204772656369616e2055726e
-// skR: efd90477fdb7b8f60357eec8d7ae348fef38b0c55c3298c09caf9d575990bd22
-// skS: 2ee3b88417a20b5fb0a527fefaae4066a6449d2d75bed96fa2478d58f300c411
-// skE: 2118dc1de1f6578b3576b4e6996fa6517ceb28a403fce626c8e0d430bd571f8b
-// psk: 3564623362383061383163623633636135393437306338333431346566373061633
-// 1636338303636333964303133353738343937343061303364616464666339
-// pskID: 456e6e796e20447572696e206172616e204d6f726961
-// pkR: 0441aa0ed8d749bab7f9a2ed9515ea60ad5b5cace45710f4ce6bf99bb44a1069d8a
-// 9c12ef2f514fb1c9185c8db167c821b2aeb38d1f821ba1164101c85ede7ee13
-// pkS: 047a9f60ef11a46a211fa3ca38c14430a282cefac5b90866918d64ffad2cdfe7d41
-// fed52aaea83f703407ed9bb3db950023a1accb689ba91b5743cec9d4680d080
-// pkE: 049904661176dd864002718fee7b491330d54f45bd37172b6b9ae8038cce88b9f9f
-// ad47829699477de2fb014827b4a8e7f1e4a870304aad3d7986d68d35cd07ff6
-// enc: 049904661176dd864002718fee7b491330d54f45bd37172b6b9ae8038cce88b9f9f
-// ad47829699477de2fb014827b4a8e7f1e4a870304aad3d7986d68d35cd07ff6
-// zz: cd6e7bb5ff8c134f2a925e9ca022e65f5b487321bc3e576f377e6f01236a1bbb
-// context: 00000100010003049904661176dd864002718fee7b491330d54f45bd37172b6
-// b9ae8038cce88b9f9fad47829699477de2fb014827b4a8e7f1e4a870304aad3d7986d68d
-// 35cd07ff60441aa0ed8d749bab7f9a2ed9515ea60ad5b5cace45710f4ce6bf99bb44a106
-// 9d8a9c12ef2f514fb1c9185c8db167c821b2aeb38d1f821ba1164101c85ede7ee1300000
-// 000000000000000000000000000000000000000000000000000000000000000000000000
-// 00000000000000000000000000000000000000000000000000000e3b0c44298fc1c149af
-// bf4c8996fb92427ae41e4649b934ca495991b7852b85555c4040629c64c5efec2f723040
-// 7d612d16289d7c5d7afcf9340280abd2de1ab
-// secret: 15a36bf657d3b3b4eb355d6bf2a595f710e4a4da37d2710964167ba8029227ee
-// key: fe8f6e7d61f81dc4cce9b185b4343323dcf7eaab8c2ac36239b2a9274c198868
-// nonce: e61fbe136571b0fa5753e51d
+(* // generated: "2764228860619e140920c7d7" *)
+(* let test1_encryption0_nonce = List.Tot.map u8_from_UInt8 [ *)
+(*   0x27uy; 0x64uy; 0x22uy; 0x88uy; 0x60uy; *)
+(*   0x61uy; 0x9euy; 0x14uy; 0x09uy; 0x20uy; *)
+(*   0xc7uy; 0xd7uy; *)
+(* ] *)
 
-let test2_ciphersuite = DH.DH_P256, AEAD.CHACHA20_POLY1305, Hash.SHA2_256
+(* // generated: "4265617574792069732074727574682c20747275746820626561757479" *)
+(* let test1_encryption0_plaintext = List.Tot.map u8_from_UInt8 [ *)
+(*   0x42uy; 0x65uy; 0x61uy; 0x75uy; 0x74uy; *)
+(*   0x79uy; 0x20uy; 0x69uy; 0x73uy; 0x20uy; *)
+(*   0x74uy; 0x72uy; 0x75uy; 0x74uy; 0x68uy; *)
+(*   0x2cuy; 0x20uy; 0x74uy; 0x72uy; 0x75uy; *)
+(*   0x74uy; 0x68uy; 0x20uy; 0x62uy; 0x65uy; *)
+(*   0x61uy; 0x75uy; 0x74uy; 0x79uy; *)
+(* ] *)
 
-let test2_info = List.Tot.map u8_from_UInt8 [
-  0x4fuy; 0x64uy; 0x65uy; 0x20uy; 0x6fuy;
-  0x6euy; 0x20uy; 0x61uy; 0x20uy; 0x47uy;
-  0x72uy; 0x65uy; 0x63uy; 0x69uy; 0x61uy;
-  0x6euy; 0x20uy; 0x55uy; 0x72uy; 0x6euy;
-]
+(* // generated: "436f756e742d31" *)
+(* let test1_encryption1_aad = List.Tot.map u8_from_UInt8 [ *)
+(*   0x43uy; 0x6fuy; 0x75uy; 0x6euy; 0x74uy; *)
+(*   0x2duy; 0x31uy; *)
+(* ] *)
 
-let test2_skR = List.Tot.map u8_from_UInt8 [
-  0xefuy; 0xd9uy; 0x04uy; 0x77uy; 0xfduy;
-  0xb7uy; 0xb8uy; 0xf6uy; 0x03uy; 0x57uy;
-  0xeeuy; 0xc8uy; 0xd7uy; 0xaeuy; 0x34uy;
-  0x8fuy; 0xefuy; 0x38uy; 0xb0uy; 0xc5uy;
-  0x5cuy; 0x32uy; 0x98uy; 0xc0uy; 0x9cuy;
-  0xafuy; 0x9duy; 0x57uy; 0x59uy; 0x90uy;
-  0xbduy; 0x22uy;
-]
+(* // generated: "2ed9ff66c33bad2f7c0326881f05aa9616ccba13bdb126a0d2a5a3dfa6b95bd4de78a98ff64c1fb64b366074d4" *)
+(* let test1_encryption1_ciphertext = List.Tot.map u8_from_UInt8 [ *)
+(*   0x2euy; 0xd9uy; 0xffuy; 0x66uy; 0xc3uy; *)
+(*   0x3buy; 0xaduy; 0x2fuy; 0x7cuy; 0x03uy; *)
+(*   0x26uy; 0x88uy; 0x1fuy; 0x05uy; 0xaauy; *)
+(*   0x96uy; 0x16uy; 0xccuy; 0xbauy; 0x13uy; *)
+(*   0xbduy; 0xb1uy; 0x26uy; 0xa0uy; 0xd2uy; *)
+(*   0xa5uy; 0xa3uy; 0xdfuy; 0xa6uy; 0xb9uy; *)
+(*   0x5buy; 0xd4uy; 0xdeuy; 0x78uy; 0xa9uy; *)
+(*   0x8fuy; 0xf6uy; 0x4cuy; 0x1fuy; 0xb6uy; *)
+(*   0x4buy; 0x36uy; 0x60uy; 0x74uy; 0xd4uy; *)
+(* ] *)
 
-let test2_skI = List.Tot.map u8_from_UInt8 [
-  0x2euy; 0xe3uy; 0xb8uy; 0x84uy; 0x17uy;
-  0xa2uy; 0x0buy; 0x5fuy; 0xb0uy; 0xa5uy;
-  0x27uy; 0xfeuy; 0xfauy; 0xaeuy; 0x40uy;
-  0x66uy; 0xa6uy; 0x44uy; 0x9duy; 0x2duy;
-  0x75uy; 0xbeuy; 0xd9uy; 0x6fuy; 0xa2uy;
-  0x47uy; 0x8duy; 0x58uy; 0xf3uy; 0x00uy;
-  0xc4uy; 0x11uy;
-]
+(* // generated: "2764228860619e140920c7d6" *)
+(* let test1_encryption1_nonce = List.Tot.map u8_from_UInt8 [ *)
+(*   0x27uy; 0x64uy; 0x22uy; 0x88uy; 0x60uy; *)
+(*   0x61uy; 0x9euy; 0x14uy; 0x09uy; 0x20uy; *)
+(*   0xc7uy; 0xd6uy; *)
+(* ] *)
 
-let test2_skE = List.Tot.map u8_from_UInt8 [
-  0x21uy; 0x18uy; 0xdcuy; 0x1duy; 0xe1uy;
-  0xf6uy; 0x57uy; 0x8buy; 0x35uy; 0x76uy;
-  0xb4uy; 0xe6uy; 0x99uy; 0x6fuy; 0xa6uy;
-  0x51uy; 0x7cuy; 0xebuy; 0x28uy; 0xa4uy;
-  0x03uy; 0xfcuy; 0xe6uy; 0x26uy; 0xc8uy;
-  0xe0uy; 0xd4uy; 0x30uy; 0xbduy; 0x57uy;
-  0x1fuy; 0x8buy;
-]
+(* // generated: "4265617574792069732074727574682c20747275746820626561757479" *)
+(* let test1_encryption1_plaintext = List.Tot.map u8_from_UInt8 [ *)
+(*   0x42uy; 0x65uy; 0x61uy; 0x75uy; 0x74uy; *)
+(*   0x79uy; 0x20uy; 0x69uy; 0x73uy; 0x20uy; *)
+(*   0x74uy; 0x72uy; 0x75uy; 0x74uy; 0x68uy; *)
+(*   0x2cuy; 0x20uy; 0x74uy; 0x72uy; 0x75uy; *)
+(*   0x74uy; 0x68uy; 0x20uy; 0x62uy; 0x65uy; *)
+(*   0x61uy; 0x75uy; 0x74uy; 0x79uy; *)
+(* ] *)
 
-let test2_psk = List.Tot.map u8_from_UInt8 [
-  0x35uy; 0x64uy; 0x62uy; 0x33uy; 0x62uy;
-  0x38uy; 0x30uy; 0x61uy; 0x38uy; 0x31uy;
-  0x63uy; 0x62uy; 0x36uy; 0x33uy; 0x63uy;
-  0x61uy; 0x35uy; 0x39uy; 0x34uy; 0x37uy;
-  0x30uy; 0x63uy; 0x38uy; 0x33uy; 0x34uy;
-  0x31uy; 0x34uy; 0x65uy; 0x66uy; 0x37uy;
-  0x30uy; 0x61uy; 0x63uy; 0x31uy; 0x63uy;
-  0x63uy; 0x38uy; 0x30uy; 0x36uy; 0x36uy;
-  0x33uy; 0x39uy; 0x64uy; 0x30uy; 0x31uy;
-  0x33uy; 0x35uy; 0x37uy; 0x38uy; 0x34uy;
-  0x39uy; 0x37uy; 0x34uy; 0x30uy; 0x61uy;
-  0x30uy; 0x33uy; 0x64uy; 0x61uy; 0x64uy;
-  0x64uy; 0x66uy; 0x63uy; 0x39uy;
-]
+(* // generated: "436f756e742d32" *)
+(* let test1_encryption2_aad = List.Tot.map u8_from_UInt8 [ *)
+(*   0x43uy; 0x6fuy; 0x75uy; 0x6euy; 0x74uy; *)
+(*   0x2duy; 0x32uy; *)
+(* ] *)
 
-let test2_pskID = List.Tot.map u8_from_UInt8 [
-  0x45uy; 0x6euy; 0x6euy; 0x79uy; 0x6euy;
-  0x20uy; 0x44uy; 0x75uy; 0x72uy; 0x69uy;
-  0x6euy; 0x20uy; 0x61uy; 0x72uy; 0x61uy;
-  0x6euy; 0x20uy; 0x4duy; 0x6fuy; 0x72uy;
-  0x69uy; 0x61uy;
-]
+(* // generated: "4bfc8da6f1da808be2c1c141e864fe536bd1e9c4e01376cd383370b8095438a06f372e663739b30af9355da8a3" *)
+(* let test1_encryption2_ciphertext = List.Tot.map u8_from_UInt8 [ *)
+(*   0x4buy; 0xfcuy; 0x8duy; 0xa6uy; 0xf1uy; *)
+(*   0xdauy; 0x80uy; 0x8buy; 0xe2uy; 0xc1uy; *)
+(*   0xc1uy; 0x41uy; 0xe8uy; 0x64uy; 0xfeuy; *)
+(*   0x53uy; 0x6buy; 0xd1uy; 0xe9uy; 0xc4uy; *)
+(*   0xe0uy; 0x13uy; 0x76uy; 0xcduy; 0x38uy; *)
+(*   0x33uy; 0x70uy; 0xb8uy; 0x09uy; 0x54uy; *)
+(*   0x38uy; 0xa0uy; 0x6fuy; 0x37uy; 0x2euy; *)
+(*   0x66uy; 0x37uy; 0x39uy; 0xb3uy; 0x0auy; *)
+(*   0xf9uy; 0x35uy; 0x5duy; 0xa8uy; 0xa3uy; *)
+(* ] *)
 
-let test2_pkR = List.Tot.map u8_from_UInt8 [
-  0x04uy; 0x41uy; 0xaauy; 0x0euy; 0xd8uy;
-  0xd7uy; 0x49uy; 0xbauy; 0xb7uy; 0xf9uy;
-  0xa2uy; 0xeduy; 0x95uy; 0x15uy; 0xeauy;
-  0x60uy; 0xaduy; 0x5buy; 0x5cuy; 0xacuy;
-  0xe4uy; 0x57uy; 0x10uy; 0xf4uy; 0xceuy;
-  0x6buy; 0xf9uy; 0x9buy; 0xb4uy; 0x4auy;
-  0x10uy; 0x69uy; 0xd8uy; 0xa9uy; 0xc1uy;
-  0x2euy; 0xf2uy; 0xf5uy; 0x14uy; 0xfbuy;
-  0x1cuy; 0x91uy; 0x85uy; 0xc8uy; 0xdbuy;
-  0x16uy; 0x7cuy; 0x82uy; 0x1buy; 0x2auy;
-  0xebuy; 0x38uy; 0xd1uy; 0xf8uy; 0x21uy;
-  0xbauy; 0x11uy; 0x64uy; 0x10uy; 0x1cuy;
-  0x85uy; 0xeduy; 0xe7uy; 0xeeuy; 0x13uy;
-]
+(* // generated: "2764228860619e140920c7d5" *)
+(* let test1_encryption2_nonce = List.Tot.map u8_from_UInt8 [ *)
+(*   0x27uy; 0x64uy; 0x22uy; 0x88uy; 0x60uy; *)
+(*   0x61uy; 0x9euy; 0x14uy; 0x09uy; 0x20uy; *)
+(*   0xc7uy; 0xd5uy; *)
+(* ] *)
 
-let test2_pkI = List.Tot.map u8_from_UInt8 [
-  0x04uy; 0x7auy; 0x9fuy; 0x60uy; 0xefuy;
-  0x11uy; 0xa4uy; 0x6auy; 0x21uy; 0x1fuy;
-  0xa3uy; 0xcauy; 0x38uy; 0xc1uy; 0x44uy;
-  0x30uy; 0xa2uy; 0x82uy; 0xceuy; 0xfauy;
-  0xc5uy; 0xb9uy; 0x08uy; 0x66uy; 0x91uy;
-  0x8duy; 0x64uy; 0xffuy; 0xaduy; 0x2cuy;
-  0xdfuy; 0xe7uy; 0xd4uy; 0x1fuy; 0xeduy;
-  0x52uy; 0xaauy; 0xeauy; 0x83uy; 0xf7uy;
-  0x03uy; 0x40uy; 0x7euy; 0xd9uy; 0xbbuy;
-  0x3duy; 0xb9uy; 0x50uy; 0x02uy; 0x3auy;
-  0x1auy; 0xccuy; 0xb6uy; 0x89uy; 0xbauy;
-  0x91uy; 0xb5uy; 0x74uy; 0x3cuy; 0xecuy;
-  0x9duy; 0x46uy; 0x80uy; 0xd0uy; 0x80uy;
-]
+(* // generated: "4265617574792069732074727574682c20747275746820626561757479" *)
+(* let test1_encryption2_plaintext = List.Tot.map u8_from_UInt8 [ *)
+(*   0x42uy; 0x65uy; 0x61uy; 0x75uy; 0x74uy; *)
+(*   0x79uy; 0x20uy; 0x69uy; 0x73uy; 0x20uy; *)
+(*   0x74uy; 0x72uy; 0x75uy; 0x74uy; 0x68uy; *)
+(*   0x2cuy; 0x20uy; 0x74uy; 0x72uy; 0x75uy; *)
+(*   0x74uy; 0x68uy; 0x20uy; 0x62uy; 0x65uy; *)
+(*   0x61uy; 0x75uy; 0x74uy; 0x79uy; *)
+(* ] *)
 
-let test2_pkE = List.Tot.map u8_from_UInt8 [
-  0x04uy; 0x99uy; 0x04uy; 0x66uy; 0x11uy;
-  0x76uy; 0xdduy; 0x86uy; 0x40uy; 0x02uy;
-  0x71uy; 0x8fuy; 0xeeuy; 0x7buy; 0x49uy;
-  0x13uy; 0x30uy; 0xd5uy; 0x4fuy; 0x45uy;
-  0xbduy; 0x37uy; 0x17uy; 0x2buy; 0x6buy;
-  0x9auy; 0xe8uy; 0x03uy; 0x8cuy; 0xceuy;
-  0x88uy; 0xb9uy; 0xf9uy; 0xfauy; 0xd4uy;
-  0x78uy; 0x29uy; 0x69uy; 0x94uy; 0x77uy;
-  0xdeuy; 0x2fuy; 0xb0uy; 0x14uy; 0x82uy;
-  0x7buy; 0x4auy; 0x8euy; 0x7fuy; 0x1euy;
-  0x4auy; 0x87uy; 0x03uy; 0x04uy; 0xaauy;
-  0xd3uy; 0xd7uy; 0x98uy; 0x6duy; 0x68uy;
-  0xd3uy; 0x5cuy; 0xd0uy; 0x7fuy; 0xf6uy;
-]
+(* // generated: "436f756e742d33" *)
+(* let test1_encryption3_aad = List.Tot.map u8_from_UInt8 [ *)
+(*   0x43uy; 0x6fuy; 0x75uy; 0x6euy; 0x74uy; *)
+(*   0x2duy; 0x33uy; *)
+(* ] *)
 
-let test2_enc = List.Tot.map u8_from_UInt8 [
-  0x04uy; 0x99uy; 0x04uy; 0x66uy; 0x11uy;
-  0x76uy; 0xdduy; 0x86uy; 0x40uy; 0x02uy;
-  0x71uy; 0x8fuy; 0xeeuy; 0x7buy; 0x49uy;
-  0x13uy; 0x30uy; 0xd5uy; 0x4fuy; 0x45uy;
-  0xbduy; 0x37uy; 0x17uy; 0x2buy; 0x6buy;
-  0x9auy; 0xe8uy; 0x03uy; 0x8cuy; 0xceuy;
-  0x88uy; 0xb9uy; 0xf9uy; 0xfauy; 0xd4uy;
-  0x78uy; 0x29uy; 0x69uy; 0x94uy; 0x77uy;
-  0xdeuy; 0x2fuy; 0xb0uy; 0x14uy; 0x82uy;
-  0x7buy; 0x4auy; 0x8euy; 0x7fuy; 0x1euy;
-  0x4auy; 0x87uy; 0x03uy; 0x04uy; 0xaauy;
-  0xd3uy; 0xd7uy; 0x98uy; 0x6duy; 0x68uy;
-  0xd3uy; 0x5cuy; 0xd0uy; 0x7fuy; 0xf6uy;
-]
+(* // generated: "cc82487c2beb92d6810a40bad2aa96794c5f2b6eff96a674cf9c9c853397e6c7ca9640c200a38326adb63ed7f2" *)
+(* let test1_encryption3_ciphertext = List.Tot.map u8_from_UInt8 [ *)
+(*   0xccuy; 0x82uy; 0x48uy; 0x7cuy; 0x2buy; *)
+(*   0xebuy; 0x92uy; 0xd6uy; 0x81uy; 0x0auy; *)
+(*   0x40uy; 0xbauy; 0xd2uy; 0xaauy; 0x96uy; *)
+(*   0x79uy; 0x4cuy; 0x5fuy; 0x2buy; 0x6euy; *)
+(*   0xffuy; 0x96uy; 0xa6uy; 0x74uy; 0xcfuy; *)
+(*   0x9cuy; 0x9cuy; 0x85uy; 0x33uy; 0x97uy; *)
+(*   0xe6uy; 0xc7uy; 0xcauy; 0x96uy; 0x40uy; *)
+(*   0xc2uy; 0x00uy; 0xa3uy; 0x83uy; 0x26uy; *)
+(*   0xaduy; 0xb6uy; 0x3euy; 0xd7uy; 0xf2uy; *)
+(* ] *)
 
-let test2_zz = List.Tot.map u8_from_UInt8 [
-  0xcduy; 0x6euy; 0x7buy; 0xb5uy; 0xffuy;
-  0x8cuy; 0x13uy; 0x4fuy; 0x2auy; 0x92uy;
-  0x5euy; 0x9cuy; 0xa0uy; 0x22uy; 0xe6uy;
-  0x5fuy; 0x5buy; 0x48uy; 0x73uy; 0x21uy;
-  0xbcuy; 0x3euy; 0x57uy; 0x6fuy; 0x37uy;
-  0x7euy; 0x6fuy; 0x01uy; 0x23uy; 0x6auy;
-  0x1buy; 0xbbuy;
-]
+(* // generated: "2764228860619e140920c7d4" *)
+(* let test1_encryption3_nonce = List.Tot.map u8_from_UInt8 [ *)
+(*   0x27uy; 0x64uy; 0x22uy; 0x88uy; 0x60uy; *)
+(*   0x61uy; 0x9euy; 0x14uy; 0x09uy; 0x20uy; *)
+(*   0xc7uy; 0xd4uy; *)
+(* ] *)
 
-let test2_context = List.Tot.map u8_from_UInt8 [
-  0x00uy; 0x00uy; 0x01uy; 0x00uy; 0x01uy;
-  0x00uy; 0x03uy; 0x04uy; 0x99uy; 0x04uy;
-  0x66uy; 0x11uy; 0x76uy; 0xdduy; 0x86uy;
-  0x40uy; 0x02uy; 0x71uy; 0x8fuy; 0xeeuy;
-  0x7buy; 0x49uy; 0x13uy; 0x30uy; 0xd5uy;
-  0x4fuy; 0x45uy; 0xbduy; 0x37uy; 0x17uy;
-  0x2buy; 0x6buy; 0x9auy; 0xe8uy; 0x03uy;
-  0x8cuy; 0xceuy; 0x88uy; 0xb9uy; 0xf9uy;
-  0xfauy; 0xd4uy; 0x78uy; 0x29uy; 0x69uy;
-  0x94uy; 0x77uy; 0xdeuy; 0x2fuy; 0xb0uy;
-  0x14uy; 0x82uy; 0x7buy; 0x4auy; 0x8euy;
-  0x7fuy; 0x1euy; 0x4auy; 0x87uy; 0x03uy;
-  0x04uy; 0xaauy; 0xd3uy; 0xd7uy; 0x98uy;
-  0x6duy; 0x68uy; 0xd3uy; 0x5cuy; 0xd0uy;
-  0x7fuy; 0xf6uy; 0x04uy; 0x41uy; 0xaauy;
-  0x0euy; 0xd8uy; 0xd7uy; 0x49uy; 0xbauy;
-  0xb7uy; 0xf9uy; 0xa2uy; 0xeduy; 0x95uy;
-  0x15uy; 0xeauy; 0x60uy; 0xaduy; 0x5buy;
-  0x5cuy; 0xacuy; 0xe4uy; 0x57uy; 0x10uy;
-  0xf4uy; 0xceuy; 0x6buy; 0xf9uy; 0x9buy;
-  0xb4uy; 0x4auy; 0x10uy; 0x69uy; 0xd8uy;
-  0xa9uy; 0xc1uy; 0x2euy; 0xf2uy; 0xf5uy;
-  0x14uy; 0xfbuy; 0x1cuy; 0x91uy; 0x85uy;
-  0xc8uy; 0xdbuy; 0x16uy; 0x7cuy; 0x82uy;
-  0x1buy; 0x2auy; 0xebuy; 0x38uy; 0xd1uy;
-  0xf8uy; 0x21uy; 0xbauy; 0x11uy; 0x64uy;
-  0x10uy; 0x1cuy; 0x85uy; 0xeduy; 0xe7uy;
-  0xeeuy; 0x13uy; 0x00uy; 0x00uy; 0x00uy;
-  0x00uy; 0x00uy; 0x00uy; 0x00uy; 0x00uy;
-  0x00uy; 0x00uy; 0x00uy; 0x00uy; 0x00uy;
-  0x00uy; 0x00uy; 0x00uy; 0x00uy; 0x00uy;
-  0x00uy; 0x00uy; 0x00uy; 0x00uy; 0x00uy;
-  0x00uy; 0x00uy; 0x00uy; 0x00uy; 0x00uy;
-  0x00uy; 0x00uy; 0x00uy; 0x00uy; 0x00uy;
-  0x00uy; 0x00uy; 0x00uy; 0x00uy; 0x00uy;
-  0x00uy; 0x00uy; 0x00uy; 0x00uy; 0x00uy;
-  0x00uy; 0x00uy; 0x00uy; 0x00uy; 0x00uy;
-  0x00uy; 0x00uy; 0x00uy; 0x00uy; 0x00uy;
-  0x00uy; 0x00uy; 0x00uy; 0x00uy; 0x00uy;
-  0x00uy; 0x00uy; 0x00uy; 0x00uy; 0x00uy;
-  0x00uy; 0x00uy; 0xe3uy; 0xb0uy; 0xc4uy;
-  0x42uy; 0x98uy; 0xfcuy; 0x1cuy; 0x14uy;
-  0x9auy; 0xfbuy; 0xf4uy; 0xc8uy; 0x99uy;
-  0x6fuy; 0xb9uy; 0x24uy; 0x27uy; 0xaeuy;
-  0x41uy; 0xe4uy; 0x64uy; 0x9buy; 0x93uy;
-  0x4cuy; 0xa4uy; 0x95uy; 0x99uy; 0x1buy;
-  0x78uy; 0x52uy; 0xb8uy; 0x55uy; 0x55uy;
-  0xc4uy; 0x04uy; 0x06uy; 0x29uy; 0xc6uy;
-  0x4cuy; 0x5euy; 0xfeuy; 0xc2uy; 0xf7uy;
-  0x23uy; 0x04uy; 0x07uy; 0xd6uy; 0x12uy;
-  0xd1uy; 0x62uy; 0x89uy; 0xd7uy; 0xc5uy;
-  0xd7uy; 0xafuy; 0xcfuy; 0x93uy; 0x40uy;
-  0x28uy; 0x0auy; 0xbduy; 0x2duy; 0xe1uy;
-  0xabuy;
-]
+(* // generated: "4265617574792069732074727574682c20747275746820626561757479" *)
+(* let test1_encryption3_plaintext = List.Tot.map u8_from_UInt8 [ *)
+(*   0x42uy; 0x65uy; 0x61uy; 0x75uy; 0x74uy; *)
+(*   0x79uy; 0x20uy; 0x69uy; 0x73uy; 0x20uy; *)
+(*   0x74uy; 0x72uy; 0x75uy; 0x74uy; 0x68uy; *)
+(*   0x2cuy; 0x20uy; 0x74uy; 0x72uy; 0x75uy; *)
+(*   0x74uy; 0x68uy; 0x20uy; 0x62uy; 0x65uy; *)
+(*   0x61uy; 0x75uy; 0x74uy; 0x79uy; *)
+(* ] *)
 
-let test2_secret = List.Tot.map u8_from_UInt8 [
-  0x15uy; 0xa3uy; 0x6buy; 0xf6uy; 0x57uy;
-  0xd3uy; 0xb3uy; 0xb4uy; 0xebuy; 0x35uy;
-  0x5duy; 0x6buy; 0xf2uy; 0xa5uy; 0x95uy;
-  0xf7uy; 0x10uy; 0xe4uy; 0xa4uy; 0xdauy;
-  0x37uy; 0xd2uy; 0x71uy; 0x09uy; 0x64uy;
-  0x16uy; 0x7buy; 0xa8uy; 0x02uy; 0x92uy;
-  0x27uy; 0xeeuy;
-]
+(* // generated: "436f756e742d34" *)
+(* let test1_encryption4_aad = List.Tot.map u8_from_UInt8 [ *)
+(*   0x43uy; 0x6fuy; 0x75uy; 0x6euy; 0x74uy; *)
+(*   0x2duy; 0x34uy; *)
+(* ] *)
 
-let test2_key = List.Tot.map u8_from_UInt8 [
-  0xfeuy; 0x8fuy; 0x6euy; 0x7duy; 0x61uy;
-  0xf8uy; 0x1duy; 0xc4uy; 0xccuy; 0xe9uy;
-  0xb1uy; 0x85uy; 0xb4uy; 0x34uy; 0x33uy;
-  0x23uy; 0xdcuy; 0xf7uy; 0xeauy; 0xabuy;
-  0x8cuy; 0x2auy; 0xc3uy; 0x62uy; 0x39uy;
-  0xb2uy; 0xa9uy; 0x27uy; 0x4cuy; 0x19uy;
-  0x88uy; 0x68uy;
-]
+(* // generated: "6314e60548cfdc30552303be4cb19875e335554bce186e1b41f9d15b4b4a4af77d68c09ebf883a9cbb51f3be9d" *)
+(* let test1_encryption4_ciphertext = List.Tot.map u8_from_UInt8 [ *)
+(*   0x63uy; 0x14uy; 0xe6uy; 0x05uy; 0x48uy; *)
+(*   0xcfuy; 0xdcuy; 0x30uy; 0x55uy; 0x23uy; *)
+(*   0x03uy; 0xbeuy; 0x4cuy; 0xb1uy; 0x98uy; *)
+(*   0x75uy; 0xe3uy; 0x35uy; 0x55uy; 0x4buy; *)
+(*   0xceuy; 0x18uy; 0x6euy; 0x1buy; 0x41uy; *)
+(*   0xf9uy; 0xd1uy; 0x5buy; 0x4buy; 0x4auy; *)
+(*   0x4auy; 0xf7uy; 0x7duy; 0x68uy; 0xc0uy; *)
+(*   0x9euy; 0xbfuy; 0x88uy; 0x3auy; 0x9cuy; *)
+(*   0xbbuy; 0x51uy; 0xf3uy; 0xbeuy; 0x9duy; *)
+(* ] *)
 
-let test2_nonce = List.Tot.map u8_from_UInt8 [
-  0xe6uy; 0x1fuy; 0xbeuy; 0x13uy; 0x65uy;
-  0x71uy; 0xb0uy; 0xfauy; 0x57uy; 0x53uy;
-  0xe5uy; 0x1duy;
-]
+(* // generated: "2764228860619e140920c7d3" *)
+(* let test1_encryption4_nonce = List.Tot.map u8_from_UInt8 [ *)
+(*   0x27uy; 0x64uy; 0x22uy; 0x88uy; 0x60uy; *)
+(*   0x61uy; 0x9euy; 0x14uy; 0x09uy; 0x20uy; *)
+(*   0xc7uy; 0xd3uy; *)
+(* ] *)
 
+(* // generated: "4265617574792069732074727574682c20747275746820626561757479" *)
+(* let test1_encryption4_plaintext = List.Tot.map u8_from_UInt8 [ *)
+(*   0x42uy; 0x65uy; 0x61uy; 0x75uy; 0x74uy; *)
+(*   0x79uy; 0x20uy; 0x69uy; 0x73uy; 0x20uy; *)
+(*   0x74uy; 0x72uy; 0x75uy; 0x74uy; 0x68uy; *)
+(*   0x2cuy; 0x20uy; 0x74uy; 0x72uy; 0x75uy; *)
+(*   0x74uy; 0x68uy; 0x20uy; 0x62uy; 0x65uy; *)
+(*   0x61uy; 0x75uy; 0x74uy; 0x79uy; *)
+(* ] *)
 
-#set-options "--ifuel 1"
-let test_base_setup
+(* // generated: "436f756e742d35" *)
+(* let test1_encryption5_aad = List.Tot.map u8_from_UInt8 [ *)
+(*   0x43uy; 0x6fuy; 0x75uy; 0x6euy; 0x74uy; *)
+(*   0x2duy; 0x35uy; *)
+(* ] *)
+
+(* // generated: "ce580d139c001ed794c4eedf14ce43c19c2a04f20dcfa9de57b6f555816b0558db4ec603bbc3748dce30e5c82f" *)
+(* let test1_encryption5_ciphertext = List.Tot.map u8_from_UInt8 [ *)
+(*   0xceuy; 0x58uy; 0x0duy; 0x13uy; 0x9cuy; *)
+(*   0x00uy; 0x1euy; 0xd7uy; 0x94uy; 0xc4uy; *)
+(*   0xeeuy; 0xdfuy; 0x14uy; 0xceuy; 0x43uy; *)
+(*   0xc1uy; 0x9cuy; 0x2auy; 0x04uy; 0xf2uy; *)
+(*   0x0duy; 0xcfuy; 0xa9uy; 0xdeuy; 0x57uy; *)
+(*   0xb6uy; 0xf5uy; 0x55uy; 0x81uy; 0x6buy; *)
+(*   0x05uy; 0x58uy; 0xdbuy; 0x4euy; 0xc6uy; *)
+(*   0x03uy; 0xbbuy; 0xc3uy; 0x74uy; 0x8duy; *)
+(*   0xceuy; 0x30uy; 0xe5uy; 0xc8uy; 0x2fuy; *)
+(* ] *)
+
+(* // generated: "2764228860619e140920c7d2" *)
+(* let test1_encryption5_nonce = List.Tot.map u8_from_UInt8 [ *)
+(*   0x27uy; 0x64uy; 0x22uy; 0x88uy; 0x60uy; *)
+(*   0x61uy; 0x9euy; 0x14uy; 0x09uy; 0x20uy; *)
+(*   0xc7uy; 0xd2uy; *)
+(* ] *)
+
+(* // generated: "4265617574792069732074727574682c20747275746820626561757479" *)
+(* let test1_encryption5_plaintext = List.Tot.map u8_from_UInt8 [ *)
+(*   0x42uy; 0x65uy; 0x61uy; 0x75uy; 0x74uy; *)
+(*   0x79uy; 0x20uy; 0x69uy; 0x73uy; 0x20uy; *)
+(*   0x74uy; 0x72uy; 0x75uy; 0x74uy; 0x68uy; *)
+(*   0x2cuy; 0x20uy; 0x74uy; 0x72uy; 0x75uy; *)
+(*   0x74uy; 0x68uy; 0x20uy; 0x62uy; 0x65uy; *)
+(*   0x61uy; 0x75uy; 0x74uy; 0x79uy; *)
+(* ] *)
+
+(* // generated: "436f756e742d36" *)
+(* let test1_encryption6_aad = List.Tot.map u8_from_UInt8 [ *)
+(*   0x43uy; 0x6fuy; 0x75uy; 0x6euy; 0x74uy; *)
+(*   0x2duy; 0x36uy; *)
+(* ] *)
+
+(* // generated: "5247db08759b2a6d9459a4cc461dfc59afb78e37b0852f9a669720df72fe5781460bcc9ae5ca00545ad06f93c3" *)
+(* let test1_encryption6_ciphertext = List.Tot.map u8_from_UInt8 [ *)
+(*   0x52uy; 0x47uy; 0xdbuy; 0x08uy; 0x75uy; *)
+(*   0x9buy; 0x2auy; 0x6duy; 0x94uy; 0x59uy; *)
+(*   0xa4uy; 0xccuy; 0x46uy; 0x1duy; 0xfcuy; *)
+(*   0x59uy; 0xafuy; 0xb7uy; 0x8euy; 0x37uy; *)
+(*   0xb0uy; 0x85uy; 0x2fuy; 0x9auy; 0x66uy; *)
+(*   0x97uy; 0x20uy; 0xdfuy; 0x72uy; 0xfeuy; *)
+(*   0x57uy; 0x81uy; 0x46uy; 0x0buy; 0xccuy; *)
+(*   0x9auy; 0xe5uy; 0xcauy; 0x00uy; 0x54uy; *)
+(*   0x5auy; 0xd0uy; 0x6fuy; 0x93uy; 0xc3uy; *)
+(* ] *)
+
+(* // generated: "2764228860619e140920c7d1" *)
+(* let test1_encryption6_nonce = List.Tot.map u8_from_UInt8 [ *)
+(*   0x27uy; 0x64uy; 0x22uy; 0x88uy; 0x60uy; *)
+(*   0x61uy; 0x9euy; 0x14uy; 0x09uy; 0x20uy; *)
+(*   0xc7uy; 0xd1uy; *)
+(* ] *)
+
+(* // generated: "4265617574792069732074727574682c20747275746820626561757479" *)
+(* let test1_encryption6_plaintext = List.Tot.map u8_from_UInt8 [ *)
+(*   0x42uy; 0x65uy; 0x61uy; 0x75uy; 0x74uy; *)
+(*   0x79uy; 0x20uy; 0x69uy; 0x73uy; 0x20uy; *)
+(*   0x74uy; 0x72uy; 0x75uy; 0x74uy; 0x68uy; *)
+(*   0x2cuy; 0x20uy; 0x74uy; 0x72uy; 0x75uy; *)
+(*   0x74uy; 0x68uy; 0x20uy; 0x62uy; 0x65uy; *)
+(*   0x61uy; 0x75uy; 0x74uy; 0x79uy; *)
+(* ] *)
+
+(* // generated: "436f756e742d37" *)
+(* let test1_encryption7_aad = List.Tot.map u8_from_UInt8 [ *)
+(*   0x43uy; 0x6fuy; 0x75uy; 0x6euy; 0x74uy; *)
+(*   0x2duy; 0x37uy; *)
+(* ] *)
+
+(* // generated: "e4ac909e74ca97d420374dba157678aad8f335b5cdaac2ca2e1813f2b3a6c0f6cfbc690dfd9b04a140861b910b" *)
+(* let test1_encryption7_ciphertext = List.Tot.map u8_from_UInt8 [ *)
+(*   0xe4uy; 0xacuy; 0x90uy; 0x9euy; 0x74uy; *)
+(*   0xcauy; 0x97uy; 0xd4uy; 0x20uy; 0x37uy; *)
+(*   0x4duy; 0xbauy; 0x15uy; 0x76uy; 0x78uy; *)
+(*   0xaauy; 0xd8uy; 0xf3uy; 0x35uy; 0xb5uy; *)
+(*   0xcduy; 0xaauy; 0xc2uy; 0xcauy; 0x2euy; *)
+(*   0x18uy; 0x13uy; 0xf2uy; 0xb3uy; 0xa6uy; *)
+(*   0xc0uy; 0xf6uy; 0xcfuy; 0xbcuy; 0x69uy; *)
+(*   0x0duy; 0xfduy; 0x9buy; 0x04uy; 0xa1uy; *)
+(*   0x40uy; 0x86uy; 0x1buy; 0x91uy; 0x0buy; *)
+(* ] *)
+
+(* // generated: "2764228860619e140920c7d0" *)
+(* let test1_encryption7_nonce = List.Tot.map u8_from_UInt8 [ *)
+(*   0x27uy; 0x64uy; 0x22uy; 0x88uy; 0x60uy; *)
+(*   0x61uy; 0x9euy; 0x14uy; 0x09uy; 0x20uy; *)
+(*   0xc7uy; 0xd0uy; *)
+(* ] *)
+
+(* // generated: "4265617574792069732074727574682c20747275746820626561757479" *)
+(* let test1_encryption7_plaintext = List.Tot.map u8_from_UInt8 [ *)
+(*   0x42uy; 0x65uy; 0x61uy; 0x75uy; 0x74uy; *)
+(*   0x79uy; 0x20uy; 0x69uy; 0x73uy; 0x20uy; *)
+(*   0x74uy; 0x72uy; 0x75uy; 0x74uy; 0x68uy; *)
+(*   0x2cuy; 0x20uy; 0x74uy; 0x72uy; 0x75uy; *)
+(*   0x74uy; 0x68uy; 0x20uy; 0x62uy; 0x65uy; *)
+(*   0x61uy; 0x75uy; 0x74uy; 0x79uy; *)
+(* ] *)
+
+(* // generated: "436f756e742d38" *)
+(* let test1_encryption8_aad = List.Tot.map u8_from_UInt8 [ *)
+(*   0x43uy; 0x6fuy; 0x75uy; 0x6euy; 0x74uy; *)
+(*   0x2duy; 0x38uy; *)
+(* ] *)
+
+(* // generated: "bd664ef7fa8fd4ba23430453914ffa75c54c24a593d894ad6626635ef38792cf505b7925d2f8dcdc744b8a8acd" *)
+(* let test1_encryption8_ciphertext = List.Tot.map u8_from_UInt8 [ *)
+(*   0xbduy; 0x66uy; 0x4euy; 0xf7uy; 0xfauy; *)
+(*   0x8fuy; 0xd4uy; 0xbauy; 0x23uy; 0x43uy; *)
+(*   0x04uy; 0x53uy; 0x91uy; 0x4fuy; 0xfauy; *)
+(*   0x75uy; 0xc5uy; 0x4cuy; 0x24uy; 0xa5uy; *)
+(*   0x93uy; 0xd8uy; 0x94uy; 0xaduy; 0x66uy; *)
+(*   0x26uy; 0x63uy; 0x5euy; 0xf3uy; 0x87uy; *)
+(*   0x92uy; 0xcfuy; 0x50uy; 0x5buy; 0x79uy; *)
+(*   0x25uy; 0xd2uy; 0xf8uy; 0xdcuy; 0xdcuy; *)
+(*   0x74uy; 0x4buy; 0x8auy; 0x8auy; 0xcduy; *)
+(* ] *)
+
+(* // generated: "2764228860619e140920c7df" *)
+(* let test1_encryption8_nonce = List.Tot.map u8_from_UInt8 [ *)
+(*   0x27uy; 0x64uy; 0x22uy; 0x88uy; 0x60uy; *)
+(*   0x61uy; 0x9euy; 0x14uy; 0x09uy; 0x20uy; *)
+(*   0xc7uy; 0xdfuy; *)
+(* ] *)
+
+(* // generated: "4265617574792069732074727574682c20747275746820626561757479" *)
+(* let test1_encryption8_plaintext = List.Tot.map u8_from_UInt8 [ *)
+(*   0x42uy; 0x65uy; 0x61uy; 0x75uy; 0x74uy; *)
+(*   0x79uy; 0x20uy; 0x69uy; 0x73uy; 0x20uy; *)
+(*   0x74uy; 0x72uy; 0x75uy; 0x74uy; 0x68uy; *)
+(*   0x2cuy; 0x20uy; 0x74uy; 0x72uy; 0x75uy; *)
+(*   0x74uy; 0x68uy; 0x20uy; 0x62uy; 0x65uy; *)
+(*   0x61uy; 0x75uy; 0x74uy; 0x79uy; *)
+(* ] *)
+
+(* // generated: "436f756e742d39" *)
+(* let test1_encryption9_aad = List.Tot.map u8_from_UInt8 [ *)
+(*   0x43uy; 0x6fuy; 0x75uy; 0x6euy; 0x74uy; *)
+(*   0x2duy; 0x39uy; *)
+(* ] *)
+
+(* // generated: "4b7f4832efecd0a808a367e4d2ac970d6604026e4386211c22912567a061a2558de77f7cb760f1837f6d048d71" *)
+(* let test1_encryption9_ciphertext = List.Tot.map u8_from_UInt8 [ *)
+(*   0x4buy; 0x7fuy; 0x48uy; 0x32uy; 0xefuy; *)
+(*   0xecuy; 0xd0uy; 0xa8uy; 0x08uy; 0xa3uy; *)
+(*   0x67uy; 0xe4uy; 0xd2uy; 0xacuy; 0x97uy; *)
+(*   0x0duy; 0x66uy; 0x04uy; 0x02uy; 0x6euy; *)
+(*   0x43uy; 0x86uy; 0x21uy; 0x1cuy; 0x22uy; *)
+(*   0x91uy; 0x25uy; 0x67uy; 0xa0uy; 0x61uy; *)
+(*   0xa2uy; 0x55uy; 0x8duy; 0xe7uy; 0x7fuy; *)
+(*   0x7cuy; 0xb7uy; 0x60uy; 0xf1uy; 0x83uy; *)
+(*   0x7fuy; 0x6duy; 0x04uy; 0x8duy; 0x71uy; *)
+(* ] *)
+
+(* // generated: "2764228860619e140920c7de" *)
+(* let test1_encryption9_nonce = List.Tot.map u8_from_UInt8 [ *)
+(*   0x27uy; 0x64uy; 0x22uy; 0x88uy; 0x60uy; *)
+(*   0x61uy; 0x9euy; 0x14uy; 0x09uy; 0x20uy; *)
+(*   0xc7uy; 0xdeuy; *)
+(* ] *)
+
+(* // generated: "4265617574792069732074727574682c20747275746820626561757479" *)
+(* let test1_encryption9_plaintext = List.Tot.map u8_from_UInt8 [ *)
+(*   0x42uy; 0x65uy; 0x61uy; 0x75uy; 0x74uy; *)
+(*   0x79uy; 0x20uy; 0x69uy; 0x73uy; 0x20uy; *)
+(*   0x74uy; 0x72uy; 0x75uy; 0x74uy; 0x68uy; *)
+(*   0x2cuy; 0x20uy; 0x74uy; 0x72uy; 0x75uy; *)
+(*   0x74uy; 0x68uy; 0x20uy; 0x62uy; 0x65uy; *)
+(*   0x61uy; 0x75uy; 0x74uy; 0x79uy; *)
+(* ] *)
+
+(* // generated: "436f6e746578742d30" *)
+(* let test1_export0_exportContext = List.Tot.map u8_from_UInt8 [ *)
+(*   0x43uy; 0x6fuy; 0x6euy; 0x74uy; 0x65uy; *)
+(*   0x78uy; 0x74uy; 0x2duy; 0x30uy; *)
+(* ] *)
+
+(* // generated: "76d8f9425846916bf678504e398e984d91878220f34c5a5e1a63ac75ba0176bc" *)
+(* let test1_export0_exportValue = List.Tot.map u8_from_UInt8 [ *)
+(*   0x76uy; 0xd8uy; 0xf9uy; 0x42uy; 0x58uy; *)
+(*   0x46uy; 0x91uy; 0x6buy; 0xf6uy; 0x78uy; *)
+(*   0x50uy; 0x4euy; 0x39uy; 0x8euy; 0x98uy; *)
+(*   0x4duy; 0x91uy; 0x87uy; 0x82uy; 0x20uy; *)
+(*   0xf3uy; 0x4cuy; 0x5auy; 0x5euy; 0x1auy; *)
+(*   0x63uy; 0xacuy; 0x75uy; 0xbauy; 0x01uy; *)
+(*   0x76uy; 0xbcuy; *)
+(* ] *)
+
+(* let test1_export0_len:size_nat = 32 *)
+(* // generated: "436f6e746578742d31" *)
+(* let test1_export1_exportContext = List.Tot.map u8_from_UInt8 [ *)
+(*   0x43uy; 0x6fuy; 0x6euy; 0x74uy; 0x65uy; *)
+(*   0x78uy; 0x74uy; 0x2duy; 0x31uy; *)
+(* ] *)
+
+(* // generated: "94fe3245047dde534862778ca1962e594b1758df5a525b4caa54ff0feadad06b" *)
+(* let test1_export1_exportValue = List.Tot.map u8_from_UInt8 [ *)
+(*   0x94uy; 0xfeuy; 0x32uy; 0x45uy; 0x04uy; *)
+(*   0x7duy; 0xdeuy; 0x53uy; 0x48uy; 0x62uy; *)
+(*   0x77uy; 0x8cuy; 0xa1uy; 0x96uy; 0x2euy; *)
+(*   0x59uy; 0x4buy; 0x17uy; 0x58uy; 0xdfuy; *)
+(*   0x5auy; 0x52uy; 0x5buy; 0x4cuy; 0xaauy; *)
+(*   0x54uy; 0xffuy; 0x0fuy; 0xeauy; 0xdauy; *)
+(*   0xd0uy; 0x6buy; *)
+(* ] *)
+
+(* let test1_export1_len:size_nat = 32 *)
+(* // generated: "436f6e746578742d32" *)
+(* let test1_export2_exportContext = List.Tot.map u8_from_UInt8 [ *)
+(*   0x43uy; 0x6fuy; 0x6euy; 0x74uy; 0x65uy; *)
+(*   0x78uy; 0x74uy; 0x2duy; 0x32uy; *)
+(* ] *)
+
+(* // generated: "97f0c64128ff1379af9ec623cba204b50cd9db9a6b7d90e7a28fed06badf363e" *)
+(* let test1_export2_exportValue = List.Tot.map u8_from_UInt8 [ *)
+(*   0x97uy; 0xf0uy; 0xc6uy; 0x41uy; 0x28uy; *)
+(*   0xffuy; 0x13uy; 0x79uy; 0xafuy; 0x9euy; *)
+(*   0xc6uy; 0x23uy; 0xcbuy; 0xa2uy; 0x04uy; *)
+(*   0xb5uy; 0x0cuy; 0xd9uy; 0xdbuy; 0x9auy; *)
+(*   0x6buy; 0x7duy; 0x90uy; 0xe7uy; 0xa2uy; *)
+(*   0x8fuy; 0xeduy; 0x06uy; 0xbauy; 0xdfuy; *)
+(*   0x36uy; 0x3euy; *)
+(* ] *)
+
+(* let test1_export2_len:size_nat = 32 *)
+(* // generated: "436f6e746578742d33" *)
+(* let test1_export3_exportContext = List.Tot.map u8_from_UInt8 [ *)
+(*   0x43uy; 0x6fuy; 0x6euy; 0x74uy; 0x65uy; *)
+(*   0x78uy; 0x74uy; 0x2duy; 0x33uy; *)
+(* ] *)
+
+(* // generated: "9cd27f832e7271f82ae85c3404d7d06ab2a5bebb9354bc022b9f016d74bcdb2c" *)
+(* let test1_export3_exportValue = List.Tot.map u8_from_UInt8 [ *)
+(*   0x9cuy; 0xd2uy; 0x7fuy; 0x83uy; 0x2euy; *)
+(*   0x72uy; 0x71uy; 0xf8uy; 0x2auy; 0xe8uy; *)
+(*   0x5cuy; 0x34uy; 0x04uy; 0xd7uy; 0xd0uy; *)
+(*   0x6auy; 0xb2uy; 0xa5uy; 0xbeuy; 0xbbuy; *)
+(*   0x93uy; 0x54uy; 0xbcuy; 0x02uy; 0x2buy; *)
+(*   0x9fuy; 0x01uy; 0x6duy; 0x74uy; 0xbcuy; *)
+(*   0xdbuy; 0x2cuy; *)
+(* ] *)
+
+(* let test1_export3_len:size_nat = 32 *)
+(* // generated: "436f6e746578742d34" *)
+(* let test1_export4_exportContext = List.Tot.map u8_from_UInt8 [ *)
+(*   0x43uy; 0x6fuy; 0x6euy; 0x74uy; 0x65uy; *)
+(*   0x78uy; 0x74uy; 0x2duy; 0x34uy; *)
+(* ] *)
+
+(* // generated: "74da0b06441dd2aca2a43d5ee4796158c9403f7037e93c50bcbd6ea4a1687c06" *)
+(* let test1_export4_exportValue = List.Tot.map u8_from_UInt8 [ *)
+(*   0x74uy; 0xdauy; 0x0buy; 0x06uy; 0x44uy; *)
+(*   0x1duy; 0xd2uy; 0xacuy; 0xa2uy; 0xa4uy; *)
+(*   0x3duy; 0x5euy; 0xe4uy; 0x79uy; 0x61uy; *)
+(*   0x58uy; 0xc9uy; 0x40uy; 0x3fuy; 0x70uy; *)
+(*   0x37uy; 0xe9uy; 0x3cuy; 0x50uy; 0xbcuy; *)
+(*   0xbduy; 0x6euy; 0xa4uy; 0xa1uy; 0x68uy; *)
+(*   0x7cuy; 0x06uy; *)
+(* ] *)
+
+(* let test1_export4_len:size_nat = 32 *)
+
+let print_and_compare_setup
   (cs:HPKE.ciphersuite)
-  (info:list uint8{List.Tot.length info <= HPKE.max_info})
-  (skR:list uint8{List.Tot.length skR == HPKE.size_dh_key cs})
-  (skI:list uint8{List.Tot.length skI == HPKE.size_dh_key cs})
-  (skE:list uint8{List.Tot.length skE == HPKE.size_dh_key cs})
-  (psk:list uint8) // {List.Tot.length psk == HPKE.size_psk cs})
-  (pskID:list uint8) //{List.Tot.length pskID <= HPKE.max_pskID})
-  (pkR:list uint8{List.Tot.length pkR == HPKE.size_dh_public cs})
-  (pkI:list uint8{List.Tot.length pkI == HPKE.size_dh_public cs})
-  (pkE:list uint8{List.Tot.length pkE == HPKE.size_dh_public cs})
-  (enc:list uint8)
-  (zz:list uint8{List.Tot.length zz == HPKE.size_dh_public cs})
-  (context:list uint8) //{List.Tot.length context == 7 + 3 * HPKE.size_dh_public cs + 2 * Hash.size_hash (HPKE.hash_of_cs cs)})
-  (secret:list uint8)
-  (key:list uint8{List.Tot.length key == HPKE.size_aead_key cs})
-  (nonce:list uint8{List.Tot.length nonce == HPKE.size_aead_nonce cs})
-= // IO.print_string "Test encap\n";
-  // let encap = HPKE.encap cs (of_list skE) (of_list pkR) in
-  // let res_encap =
-  //   if None? encap then (
-  //      IO.print_string "encap returned None\n"; false
-  //   ) else (
-  //     let (returned_zz, returned_pkE) = Some?.v encap in
-  //     let r2_a = for_all2 (fun a b -> uint_to_nat #U8 a = uint_to_nat #U8 b)
-  //       (of_list pkE) returned_pkE in
-  //     let r2_b = for_all2 (fun a b -> uint_to_nat #U8 a = uint_to_nat #U8 b)
-  //       (of_list zz) returned_zz in
-  //     if not r2_a then (
-  //       IO.print_string "\nExpected pkE :";
-  //       List.iter (fun a -> IO.print_string (UInt8.to_string (u8_to_UInt8 a))) pkE;
-  //       IO.print_string "\nComputed pkE :";
-  //       List.iter (fun a -> IO.print_string (UInt8.to_string (u8_to_UInt8 a))) (to_list returned_pkE);
-  //       IO.print_string "\n");
-  //     if not r2_b then (
-  //       IO.print_string "\nExpected zz :";
-  //       List.iter (fun a -> IO.print_string (UInt8.to_string (u8_to_UInt8 a))) zz;
-  //       IO.print_string "\nComputed zz :";
-  //       List.iter (fun a -> IO.print_string (UInt8.to_string (u8_to_UInt8 a))) (to_list returned_zz);
-  //       IO.print_string "\n");
-  //     r2_a && r2_b
-  //   )
-
-  // in
-
-  // IO.print_string "Test ks_derive\n";
-
-  // let (psk, pskID) = (HPKE.default_psk cs, HPKE.default_pskId) in
-  // let pkI = HPKE.default_pkI cs in
-  // let pskID_hash = Hash.hash (HPKE.hash_of_cs cs) pskID in
-  // let info_hash = Hash.hash (HPKE.hash_of_cs cs) (of_list info) in
-  // let returned_context = HPKE.build_context HPKE.Base cs (of_list pkE) (of_list pkR) pkI pskID_hash info_hash in
+  (enc:HPKE.key_dh_public_s cs)
+  (key:HPKE.key_aead_s cs) (nonce:HPKE.nonce_aead_s cs) (exp_sec:HPKE.exporter_secret_s cs)
+  (enc_i:HPKE.key_dh_public_s cs) (ctx_i:HPKE.encryption_context cs)
+=
+  let r1 = print_and_compare_bytes (HPKE.size_dh_public cs) enc enc_i in
+  let r2 = print_and_compare_bytes (HPKE.size_aead_key cs) key (HPKE.key_of_ctx cs ctx_i) in
+  let r3 = print_and_compare_bytes (HPKE.size_aead_nonce cs) nonce (HPKE.nonce_of_ctx cs ctx_i) in
+  let r4 = print_and_compare_bytes (HPKE.size_kdf cs) exp_sec (HPKE.exp_sec_of_ctx cs ctx_i) in
+  r1 && r2 && r3 && r4
 
 
-  // IO.print_string "\nExpected context :";
-  // List.iter (fun a -> IO.print_string (UInt8.to_string (u8_to_UInt8 a))) context;
-  // IO.print_string "\nComputed context :";
-  // List.iter (fun a -> IO.print_string (UInt8.to_string (u8_to_UInt8 a))) (to_list returned_context);
-  // IO.print_string "\n";
+let test_setupBase
+  (cs:HPKE.ciphersuite)
+  (skEm:HPKE.key_dh_secret_s cs) (pkEm:HPKE.key_dh_public_s cs) (skRm:HPKE.key_dh_secret_s cs) (pkRm:HPKE.key_dh_public_s cs) (info:HPKE.info_s cs)
+  (enc:HPKE.key_dh_public_s cs) (zz:HPKE.key_kem_s cs)
+  (ks_context:lbytes (HPKE.size_ks_ctx cs)) (secret:lbytes (HPKE.size_kdf cs))
+  (key:HPKE.key_aead_s cs) (nonce:HPKE.nonce_aead_s cs) (exp_sec:HPKE.exporter_secret_s cs)
+  (enc0_nonce:HPKE.nonce_aead_s cs) (enc1_nonce:HPKE.nonce_aead_s cs)
+=
+  print "Test setupBaseS\n";
+  let pkR = HPKE.unmarshal cs pkRm in
+  match HPKE.setupBaseS cs skEm pkR info with
+  | None -> false
+  | Some (enc_i, ctx_i) -> print_and_compare_setup cs enc key nonce exp_sec enc_i ctx_i
 
-  // let returned_secret = HKDF.extract (HPKE.hash_of_cs cs) psk (of_list zz) in
+let test_export
+  (cs:HPKE.ciphersuite)
+  (key:HPKE.key_aead_s cs) (nonce:HPKE.nonce_aead_s cs) (exp_sec:HPKE.exporter_secret_s cs)
+  (exp_ctx:HPKE.exp_ctx_s cs)
+  (exp_len:size_nat{HKDF.expand_output_length_pred (HPKE.hash_of_cs cs) exp_len})
+  (sec:lbytes exp_len)
+=
+  print "Test export\n";
+  let ctx:(HPKE.encryption_context cs) = (key, nonce, 0, exp_sec) in
+  let sec_i = HPKE.context_export cs ctx exp_ctx exp_len in
+  let r = print_and_compare_bytes exp_len sec sec_i in
+  r
 
-  // IO.print_string "\nExpected secret :";
-  // List.iter (fun a -> IO.print_string (UInt8.to_string (u8_to_UInt8 a))) secret;
-  // IO.print_string "\nComputed secret :";
-  // List.iter (fun a -> IO.print_string (UInt8.to_string (u8_to_UInt8 a))) (to_list returned_secret);
-  // IO.print_string "\n";
+let test_encryption
+  (cs:HPKE.ciphersuite)
+  (key:HPKE.key_aead_s cs) (nonce:HPKE.nonce_aead_s cs) (exp_sec:HPKE.exporter_secret_s cs)
+  (aad:AEAD.ad (HPKE.aead_of_cs cs)) (pt:AEAD.plain (HPKE.aead_of_cs cs)) (seq:HPKE.seq_aead_s cs)
+  (ct:AEAD.cipher (HPKE.aead_of_cs cs)) (enc_nonce:HPKE.nonce_aead_s cs)
+=
+  print "Test encryption\n";
+  let ctx:(HPKE.encryption_context cs) = (key, nonce, seq, exp_sec) in
+  let enc_nonce_i = HPKE.context_compute_nonce cs ctx seq in
+  print_and_compare_bytes (HPKE.size_aead_nonce cs) enc_nonce enc_nonce_i
 
+(* #set-options "--ifuel 1" *)
+(* let test_base_setup *)
+(*   (cs:HPKE.ciphersuite) *)
+(*   (info:list uint8{List.Tot.length info <= HPKE.max_info cs}) *)
+(*   (skR:list uint8{List.Tot.length skR == HPKE.size_dh_key cs}) *)
+(*   (skI:list uint8{List.Tot.length skI == HPKE.size_dh_key cs}) *)
+(*   (skE:list uint8{List.Tot.length skE == HPKE.size_dh_key cs}) *)
+(*   (psk:list uint8) // {List.Tot.length psk == HPKE.size_psk cs}) *)
+(*   (pskID:list uint8) //{List.Tot.length pskID <= HPKE.max_pskID}) *)
+(*   (pkR:list uint8{List.Tot.length pkR == HPKE.size_dh_public cs}) *)
+(*   (pkI:list uint8{List.Tot.length pkI == HPKE.size_dh_public cs}) *)
+(*   (pkE:list uint8{List.Tot.length pkE == HPKE.size_dh_public cs}) *)
+(*   (enc:list uint8) *)
+(*   (zz:list uint8{List.Tot.length zz == HPKE.size_dh_public cs}) *)
+(*   (context:list uint8) //{List.Tot.length context == 7 + 3 * HPKE.size_dh_public cs + 2 * Hash.size_hash (HPKE.hash_of_cs cs)}) *)
+(*   (secret:list uint8) *)
+(*   (key:list uint8{List.Tot.length key == HPKE.size_aead_key cs}) *)
+(*   (nonce:list uint8{List.Tot.length nonce == HPKE.size_aead_nonce cs}) *)
+(* = // IO.print_string "Test encap\n"; *)
+(*   // let encap = HPKE.encap cs (of_list skE) (of_list pkR) in *)
+(*   // let res_encap = *)
+(*   //   if None? encap then ( *)
+(*   //      IO.print_string "encap returned None\n"; false *)
+(*   //   ) else ( *)
+(*   //     let (returned_zz, returned_pkE) = Some?.v encap in *)
+(*   //     let r2_a = for_all2 (fun a b -> uint_to_nat #U8 a = uint_to_nat #U8 b) *)
+(*   //       (of_list pkE) returned_pkE in *)
+(*   //     let r2_b = for_all2 (fun a b -> uint_to_nat #U8 a = uint_to_nat #U8 b) *)
+(*   //       (of_list zz) returned_zz in *)
+(*   //     if not r2_a then ( *)
+(*   //       IO.print_string "\nExpected pkE :"; *)
+(*   //       List.iter (fun a -> IO.print_string (UInt8.to_string (u8_to_UInt8 a))) pkE; *)
+(*   //       IO.print_string "\nComputed pkE :"; *)
+(*   //       List.iter (fun a -> IO.print_string (UInt8.to_string (u8_to_UInt8 a))) (to_list returned_pkE); *)
+(*   //       IO.print_string "\n"); *)
+(*   //     if not r2_b then ( *)
+(*   //       IO.print_string "\nExpected zz :"; *)
+(*   //       List.iter (fun a -> IO.print_string (UInt8.to_string (u8_to_UInt8 a))) zz; *)
+(*   //       IO.print_string "\nComputed zz :"; *)
+(*   //       List.iter (fun a -> IO.print_string (UInt8.to_string (u8_to_UInt8 a))) (to_list returned_zz); *)
+(*   //       IO.print_string "\n"); *)
+(*   //     r2_a && r2_b *)
+(*   //   ) *)
 
-  // let info_key = Seq.append HPKE.label_key (of_list context) in
-  // let info_nonce = Seq.append HPKE.label_nonce (of_list context) in
-  // let keyIR = HKDF.expand (HPKE.hash_of_cs cs) returned_secret info_key (HPKE.size_aead_key cs) in
-  // let nonceIR = HKDF.expand (HPKE.hash_of_cs cs) returned_secret info_nonce (HPKE.size_aead_nonce cs) in
+(*   // in *)
 
-  // IO.print_string "\nExpected key :";
-  // List.iter (fun a -> IO.print_string (UInt8.to_string (u8_to_UInt8 a))) key;
-  // IO.print_string "\nComputed key :";
-  // List.iter (fun a -> IO.print_string (UInt8.to_string (u8_to_UInt8 a))) (to_list keyIR);
-  // IO.print_string "\n";
+(*   // IO.print_string "Test ks_derive\n"; *)
 
-  // IO.print_string "\nExpected nonce :";
-  // List.iter (fun a -> IO.print_string (UInt8.to_string (u8_to_UInt8 a))) nonce;
-  // IO.print_string "\nComputed nonce :";
-  // List.iter (fun a -> IO.print_string (UInt8.to_string (u8_to_UInt8 a))) (to_list nonceIR);
-  // IO.print_string "\n";
-
-
-
-  // let k, n = HPKE.ks_derive cs HPKE.Base (of_list pkR) (of_list zz) (of_list pkE)
-  //   (of_list info) None None in
-
-  IO.print_string "Test setupBaseS\n";
-  let setupBaseS = HPKE.setupBaseS cs (of_list skE) (of_list pkR) (of_list info) in
-  let res_setupBaseS =
-    if None? setupBaseS then (
-      IO.print_string "setupBaseS returned None\n"; false
-    ) else (
-      let returned_pkE, returned_key, returned_nonce = Some?.v setupBaseS in
-      let r2_a = for_all2 (fun a b -> uint_to_nat #U8 a = uint_to_nat #U8 b)
-        (of_list pkE) returned_pkE in
-      let r2_b = for_all2 (fun a b -> uint_to_nat #U8 a = uint_to_nat #U8 b)
-        (of_list key) returned_key in
-      let r2_c = for_all2 (fun a b -> uint_to_nat #U8 a = uint_to_nat #U8 b)
-        (of_list nonce) returned_nonce in
-      if not r2_a then (
-        IO.print_string "\nExpected pkE :";
-        List.iter (fun a -> IO.print_string (UInt8.to_string (u8_to_UInt8 a))) pkE;
-        IO.print_string "\nComputed pkE :";
-        List.iter (fun a -> IO.print_string (UInt8.to_string (u8_to_UInt8 a))) (to_list returned_pkE);
-        IO.print_string "\n");
-      if not r2_b then (
-        IO.print_string "\nExpected key :";
-        List.iter (fun a -> IO.print_string (UInt8.to_string (u8_to_UInt8 a))) key;
-        IO.print_string "\nComputed key :";
-        List.iter (fun a -> IO.print_string (UInt8.to_string (u8_to_UInt8 a))) (to_list returned_key);
-        IO.print_string "\n");
-      if not r2_c then (
-        IO.print_string "\nExpected nonce :";
-        List.iter (fun a -> IO.print_string (UInt8.to_string (u8_to_UInt8 a))) nonce;
-        IO.print_string "\nComputed nonce :";
-        List.iter (fun a -> IO.print_string (UInt8.to_string (u8_to_UInt8 a))) (to_list returned_nonce);
-        IO.print_string "\n");
-
-      r2_a && r2_b && r2_c
-    )
-  in
-
-  if res_setupBaseS then IO.print_string "setupBaseS succeeded\n" else IO.print_string "setupBaseS failed\n";
-
-  IO.print_string "Test setupBaseR\n";
-  let setupBaseR = HPKE.setupBaseR cs (of_list pkE) (of_list skR) (of_list info) in
-  let res_setupBaseR =
-    if None? setupBaseR then (
-      IO.print_string "setupBaseR returned None\n"; false
-    ) else (
-      let returned_key, returned_nonce = Some?.v setupBaseR in
-      let r2_a = for_all2 (fun a b -> uint_to_nat #U8 a = uint_to_nat #U8 b)
-        (of_list key) returned_key in
-      let r2_b = for_all2 (fun a b -> uint_to_nat #U8 a = uint_to_nat #U8 b)
-        (of_list nonce) returned_nonce in
-      if not r2_a then (
-        IO.print_string "\nExpected key :";
-        List.iter (fun a -> IO.print_string (UInt8.to_string (u8_to_UInt8 a))) key;
-        IO.print_string "\nComputed key :";
-        List.iter (fun a -> IO.print_string (UInt8.to_string (u8_to_UInt8 a))) (to_list returned_key);
-        IO.print_string "\n");
-      if not r2_b then (
-        IO.print_string "\nExpected nonce :";
-        List.iter (fun a -> IO.print_string (UInt8.to_string (u8_to_UInt8 a))) nonce;
-        IO.print_string "\nComputed nonce :";
-        List.iter (fun a -> IO.print_string (UInt8.to_string (u8_to_UInt8 a))) (to_list returned_nonce);
-        IO.print_string "\n");
-
-      r2_a && r2_b
-    )
-  in
-
-  if res_setupBaseR then IO.print_string "setupBaseR succeeded\n" else IO.print_string "setupBaseR failed\n";
-
-  res_setupBaseS && res_setupBaseR
-
-let test_encrytion (cs:HPKE.ciphersuite)
-  (skE:list uint8{List.Tot.length skE == HPKE.size_dh_key cs})
-  (skR:list uint8{List.Tot.length skR == HPKE.size_dh_key cs})
-  (pkR:list uint8{List.Tot.length pkR == HPKE.size_dh_public cs})
-  (pkE:list uint8{List.Tot.length pkE == HPKE.size_dh_public cs})
-  (plain:list uint8{List.Tot.length plain <= HPKE.max_length cs})
-  (aad:list uint8{List.Tot.length aad <= HPKE.max_info})
-  (cipher:list uint8{
-    List.Tot.length cipher + HPKE.size_dh_public cs <= max_size_t /\
-    List.Tot.length cipher == AEAD.cipher_length #(HPKE.aead_of_cs cs) (of_list plain)})
-  =
-  let clength = HPKE.size_dh_public cs + List.Tot.length cipher in
-  let expected_pkcipher:lbytes clength = Seq.append (of_list pkE) (of_list cipher) in
+(*   // let (psk, pskID) = (HPKE.default_psk cs, HPKE.default_pskId) in *)
+(*   // let pkI = HPKE.default_pkI cs in *)
+(*   // let pskID_hash = Hash.hash (HPKE.hash_of_cs cs) pskID in *)
+(*   // let info_hash = Hash.hash (HPKE.hash_of_cs cs) (of_list info) in *)
+(*   // let returned_context = HPKE.build_context HPKE.Base cs (of_list pkE) (of_list pkR) pkI pskID_hash info_hash in *)
 
 
-  let sealBase = HPKE.sealBase cs (of_list skE) (of_list pkR) (of_list plain) (of_list aad) in
-  let res_sealBase =
-    if None? sealBase then (
-      IO.print_string "sealBase returned None\n"; false
-    ) else (
-      let returned_pkcipher:lbytes clength = Some?.v sealBase in
-      let res = for_all2 (fun a b -> uint_to_nat #U8 a = uint_to_nat #U8 b)
-        expected_pkcipher returned_pkcipher in
-      if not res then (
-        IO.print_string "\nExpected pkE + cipher :";
-        List.iter (fun a -> IO.print_string (UInt8.to_string (u8_to_UInt8 a))) (to_list expected_pkcipher);
-        IO.print_string "\nComputed pkE + cipher :";
-        List.iter (fun a -> IO.print_string (UInt8.to_string (u8_to_UInt8 a))) (to_list returned_pkcipher);
-        IO.print_string "\n");
-       res
-     )
-  in
+(*   // IO.print_string "\nExpected context :"; *)
+(*   // List.iter (fun a -> IO.print_string (UInt8.to_string (u8_to_UInt8 a))) context; *)
+(*   // IO.print_string "\nComputed context :"; *)
+(*   // List.iter (fun a -> IO.print_string (UInt8.to_string (u8_to_UInt8 a))) (to_list returned_context); *)
+(*   // IO.print_string "\n"; *)
 
-  if res_sealBase then IO.print_string "sealBase succeeded\n" else IO.print_string "sealBase failed\n";
+(*   // let returned_secret = HKDF.extract (HPKE.hash_of_cs cs) psk (of_list zz) in *)
 
-  let openBase = HPKE.openBase cs (of_list skR) expected_pkcipher (of_list aad) in
-  let res_openBase =
-    if None? openBase then (
-      IO.print_string "openBase returned None\n"; false
-    ) else (
-      let returned_plain:lbytes (List.Tot.length plain) = Some?.v openBase in
-      let res = for_all2 (fun a b -> uint_to_nat #U8 a = uint_to_nat #U8 b)
-        (of_list plain) returned_plain in
-      if not res then (
-        IO.print_string "\nExpected plain :";
-        List.iter (fun a -> IO.print_string (UInt8.to_string (u8_to_UInt8 a))) plain;
-        IO.print_string "\nComputed plain :";
-        List.iter (fun a -> IO.print_string (UInt8.to_string (u8_to_UInt8 a))) (to_list returned_plain);
-        IO.print_string "\n");
-       res
-     )
-  in
-
-  if res_openBase then IO.print_string "openBase succeeded\n" else IO.print_string "openBase failed\n";
+(*   // IO.print_string "\nExpected secret :"; *)
+(*   // List.iter (fun a -> IO.print_string (UInt8.to_string (u8_to_UInt8 a))) secret; *)
+(*   // IO.print_string "\nComputed secret :"; *)
+(*   // List.iter (fun a -> IO.print_string (UInt8.to_string (u8_to_UInt8 a))) (to_list returned_secret); *)
+(*   // IO.print_string "\n"; *)
 
 
-  res_sealBase && res_openBase
+(*   // let info_key = Seq.append HPKE.label_key (of_list context) in *)
+(*   // let info_nonce = Seq.append HPKE.label_nonce (of_list context) in *)
+(*   // let keyIR = HKDF.expand (HPKE.hash_of_cs cs) returned_secret info_key (HPKE.size_aead_key cs) in *)
+(*   // let nonceIR = HKDF.expand (HPKE.hash_of_cs cs) returned_secret info_nonce (HPKE.size_aead_nonce cs) in *)
+
+(*   // IO.print_string "\nExpected key :"; *)
+(*   // List.iter (fun a -> IO.print_string (UInt8.to_string (u8_to_UInt8 a))) key; *)
+(*   // IO.print_string "\nComputed key :"; *)
+(*   // List.iter (fun a -> IO.print_string (UInt8.to_string (u8_to_UInt8 a))) (to_list keyIR); *)
+(*   // IO.print_string "\n"; *)
+
+(*   // IO.print_string "\nExpected nonce :"; *)
+(*   // List.iter (fun a -> IO.print_string (UInt8.to_string (u8_to_UInt8 a))) nonce; *)
+(*   // IO.print_string "\nComputed nonce :"; *)
+(*   // List.iter (fun a -> IO.print_string (UInt8.to_string (u8_to_UInt8 a))) (to_list nonceIR); *)
+(*   // IO.print_string "\n"; *)
+
+
+
+(*   // let k, n = HPKE.ks_derive cs HPKE.Base (of_list pkR) (of_list zz) (of_list pkE) *)
+(*   //   (of_list info) None None in *)
+
+(*   IO.print_string "Test setupBaseS\n"; *)
+(*   let setupBaseS = HPKE.setupBaseS cs (of_list skE) (of_list pkR) (of_list info) in *)
+(*   let res_setupBaseS = *)
+(*     if None? setupBaseS then ( *)
+(*       IO.print_string "setupBaseS returned None\n"; false *)
+(*     ) else ( *)
+(*       let returned_pkE, returned_key, returned_nonce = Some?.v setupBaseS in *)
+(*       let r2_a = for_all2 (fun a b -> uint_to_nat #U8 a = uint_to_nat #U8 b) *)
+(*         (of_list pkE) returned_pkE in *)
+(*       let r2_b = for_all2 (fun a b -> uint_to_nat #U8 a = uint_to_nat #U8 b) *)
+(*         (of_list key) returned_key in *)
+(*       let r2_c = for_all2 (fun a b -> uint_to_nat #U8 a = uint_to_nat #U8 b) *)
+(*         (of_list nonce) returned_nonce in *)
+(*       if not r2_a then ( *)
+(*         IO.print_string "\nExpected pkE :"; *)
+(*         List.iter (fun a -> IO.print_string (UInt8.to_string (u8_to_UInt8 a))) pkE; *)
+(*         IO.print_string "\nComputed pkE :"; *)
+(*         List.iter (fun a -> IO.print_string (UInt8.to_string (u8_to_UInt8 a))) (to_list returned_pkE); *)
+(*         IO.print_string "\n"); *)
+(*       if not r2_b then ( *)
+(*         IO.print_string "\nExpected key :"; *)
+(*         List.iter (fun a -> IO.print_string (UInt8.to_string (u8_to_UInt8 a))) key; *)
+(*         IO.print_string "\nComputed key :"; *)
+(*         List.iter (fun a -> IO.print_string (UInt8.to_string (u8_to_UInt8 a))) (to_list returned_key); *)
+(*         IO.print_string "\n"); *)
+(*       if not r2_c then ( *)
+(*         IO.print_string "\nExpected nonce :"; *)
+(*         List.iter (fun a -> IO.print_string (UInt8.to_string (u8_to_UInt8 a))) nonce; *)
+(*         IO.print_string "\nComputed nonce :"; *)
+(*         List.iter (fun a -> IO.print_string (UInt8.to_string (u8_to_UInt8 a))) (to_list returned_nonce); *)
+(*         IO.print_string "\n"); *)
+
+(*       r2_a && r2_b && r2_c *)
+(*     ) *)
+(*   in *)
+
+(*   if res_setupBaseS then IO.print_string "setupBaseS succeeded\n" else IO.print_string "setupBaseS failed\n"; *)
+
+(*   IO.print_string "Test setupBaseR\n"; *)
+(*   let setupBaseR = HPKE.setupBaseR cs (of_list pkE) (of_list skR) (of_list info) in *)
+(*   let res_setupBaseR = *)
+(*     if None? setupBaseR then ( *)
+(*       IO.print_string "setupBaseR returned None\n"; false *)
+(*     ) else ( *)
+(*       let returned_key, returned_nonce = Some?.v setupBaseR in *)
+(*       let r2_a = for_all2 (fun a b -> uint_to_nat #U8 a = uint_to_nat #U8 b) *)
+(*         (of_list key) returned_key in *)
+(*       let r2_b = for_all2 (fun a b -> uint_to_nat #U8 a = uint_to_nat #U8 b) *)
+(*         (of_list nonce) returned_nonce in *)
+(*       if not r2_a then ( *)
+(*         IO.print_string "\nExpected key :"; *)
+(*         List.iter (fun a -> IO.print_string (UInt8.to_string (u8_to_UInt8 a))) key; *)
+(*         IO.print_string "\nComputed key :"; *)
+(*         List.iter (fun a -> IO.print_string (UInt8.to_string (u8_to_UInt8 a))) (to_list returned_key); *)
+(*         IO.print_string "\n"); *)
+(*       if not r2_b then ( *)
+(*         IO.print_string "\nExpected nonce :"; *)
+(*         List.iter (fun a -> IO.print_string (UInt8.to_string (u8_to_UInt8 a))) nonce; *)
+(*         IO.print_string "\nComputed nonce :"; *)
+(*         List.iter (fun a -> IO.print_string (UInt8.to_string (u8_to_UInt8 a))) (to_list returned_nonce); *)
+(*         IO.print_string "\n"); *)
+
+(*       r2_a && r2_b *)
+(*     ) *)
+(*   in *)
+
+(*   if res_setupBaseR then IO.print_string "setupBaseR succeeded\n" else IO.print_string "setupBaseR failed\n"; *)
+
+(*   res_setupBaseS && res_setupBaseR *)
+
+(* let test_encrytion (cs:HPKE.ciphersuite) *)
+(*   (skE:list uint8{List.Tot.length skE == HPKE.size_dh_key cs}) *)
+(*   (skR:list uint8{List.Tot.length skR == HPKE.size_dh_key cs}) *)
+(*   (pkR:list uint8{List.Tot.length pkR == HPKE.size_dh_public cs}) *)
+(*   (pkE:list uint8{List.Tot.length pkE == HPKE.size_dh_public cs}) *)
+(*   (plain:list uint8{List.Tot.length plain <= HPKE.max_length cs}) *)
+(*   (aad:list uint8{List.Tot.length aad <= HPKE.max_info}) *)
+(*   (cipher:list uint8{ *)
+(*     List.Tot.length cipher + HPKE.size_dh_public cs <= max_size_t /\ *)
+(*     List.Tot.length cipher == AEAD.cipher_length #(HPKE.aead_of_cs cs) (of_list plain)}) *)
+(*   = *)
+(*   let clength = HPKE.size_dh_public cs + List.Tot.length cipher in *)
+(*   let expected_pkcipher:lbytes clength = Seq.append (of_list pkE) (of_list cipher) in *)
+
+
+(*   let sealBase = HPKE.sealBase cs (of_list skE) (of_list pkR) (of_list plain) (of_list aad) in *)
+(*   let res_sealBase = *)
+(*     if None? sealBase then ( *)
+(*       IO.print_string "sealBase returned None\n"; false *)
+(*     ) else ( *)
+(*       let returned_pkcipher:lbytes clength = Some?.v sealBase in *)
+(*       let res = for_all2 (fun a b -> uint_to_nat #U8 a = uint_to_nat #U8 b) *)
+(*         expected_pkcipher returned_pkcipher in *)
+(*       if not res then ( *)
+(*         IO.print_string "\nExpected pkE + cipher :"; *)
+(*         List.iter (fun a -> IO.print_string (UInt8.to_string (u8_to_UInt8 a))) (to_list expected_pkcipher); *)
+(*         IO.print_string "\nComputed pkE + cipher :"; *)
+(*         List.iter (fun a -> IO.print_string (UInt8.to_string (u8_to_UInt8 a))) (to_list returned_pkcipher); *)
+(*         IO.print_string "\n"); *)
+(*        res *)
+(*      ) *)
+(*   in *)
+
+(*   if res_sealBase then IO.print_string "sealBase succeeded\n" else IO.print_string "sealBase failed\n"; *)
+
+(*   let openBase = HPKE.openBase cs (of_list skR) expected_pkcipher (of_list aad) in *)
+(*   let res_openBase = *)
+(*     if None? openBase then ( *)
+(*       IO.print_string "openBase returned None\n"; false *)
+(*     ) else ( *)
+(*       let returned_plain:lbytes (List.Tot.length plain) = Some?.v openBase in *)
+(*       let res = for_all2 (fun a b -> uint_to_nat #U8 a = uint_to_nat #U8 b) *)
+(*         (of_list plain) returned_plain in *)
+(*       if not res then ( *)
+(*         IO.print_string "\nExpected plain :"; *)
+(*         List.iter (fun a -> IO.print_string (UInt8.to_string (u8_to_UInt8 a))) plain; *)
+(*         IO.print_string "\nComputed plain :"; *)
+(*         List.iter (fun a -> IO.print_string (UInt8.to_string (u8_to_UInt8 a))) (to_list returned_plain); *)
+(*         IO.print_string "\n"); *)
+(*        res *)
+(*      ) *)
+(*   in *)
+
+(*   if res_openBase then IO.print_string "openBase succeeded\n" else IO.print_string "openBase failed\n"; *)
+
+
+(*   res_sealBase && res_openBase *)
 
 
 //
 // Main
 //
+
 let test1 () =
-  IO.print_string "\nTest 1\n";
+  let res = test_setupBase test1_ciphersuite test1_skEm test1_pkEm test1_skRm test1_pkRm test1_info test1_enc test1_zz test1_key_schedule_context test1_secret test1_key test1_nonce test1_exporterSecret test1_encryption0_nonce test1_encryption1_nonce in
+  let seq0:HPKE.seq_aead_s test1_ciphersuite = 0 in
+  let enc_res0 = test_encryption test1_ciphersuite test1_key test1_nonce test1_exporterSecret test1_encryption0_aad test1_encryption0_plaintext seq0 test1_encryption0_ciphertext test1_encryption0_nonce in
+  assert_norm (1 < pow2 (8 * 12));
+  let seq1:HPKE.seq_aead_s test1_ciphersuite = (seq0 + 1) in
+  let enc_res1 = test_encryption test1_ciphersuite test1_key test1_nonce test1_exporterSecret test1_encryption1_aad test1_encryption1_plaintext seq1 test1_encryption1_ciphertext test1_encryption1_nonce in
+  (* let enc_res2 = test_encryption test1_ciphersuite test1_key test1_nonce test1_exporterSecret test1_encryption2_aad test1_encryption2_plaintext 2 test1_encryption2_ciphertext test1_encryption2_nonce in *)
+  (* let enc_res3 = test_encryption test1_ciphersuite test1_key test1_nonce test1_exporterSecret test1_encryption3_aad test1_encryption3_plaintext 3 test1_encryption3_ciphertext test1_encryption3_nonce in *)
+  (* let enc_res4 = test_encryption test1_ciphersuite test1_key test1_nonce test1_exporterSecret test1_encryption4_aad test1_encryption4_plaintext 4 test1_encryption4_ciphertext test1_encryption4_nonce in *)
+  (* let enc_res5 = test_encryption test1_ciphersuite test1_key test1_nonce test1_exporterSecret test1_encryption5_aad test1_encryption5_plaintext 5 test1_encryption5_ciphertext test1_encryption5_nonce in *)
+  (* let enc_res6 = test_encryption test1_ciphersuite test1_key test1_nonce test1_exporterSecret test1_encryption6_aad test1_encryption6_plaintext 6 test1_encryption6_ciphertext test1_encryption6_nonce in *)
+  (* let enc_res7 = test_encryption test1_ciphersuite test1_key test1_nonce test1_exporterSecret test1_encryption7_aad test1_encryption7_plaintext 7 test1_encryption7_ciphertext test1_encryption7_nonce in *)
+  (* let enc_res8 = test_encryption test1_ciphersuite test1_key test1_nonce test1_exporterSecret test1_encryption8_aad test1_encryption8_plaintext 8 test1_encryption8_ciphertext test1_encryption8_nonce in *)
+  (* let enc_res9 = test_encryption test1_ciphersuite test1_key test1_nonce test1_exporterSecret test1_encryption9_aad test1_encryption9_plaintext 9 test1_encryption9_ciphertext test1_encryption9_nonce in *)
+  let exp_res0 = test_export test1_ciphersuite test1_key test1_nonce test1_exporterSecret test1_export0_exportContext test1_export0_len test1_export0_exportValue in
+  (* let exp_res1 = test_export test1_ciphersuite test1_key test1_nonce test1_exporterSecret test1_export1_exportContext test1_export1_len test1_export1_exportValue in *)
+  (* let exp_res2 = test_export test1_ciphersuite test1_key test1_nonce test1_exporterSecret test1_export2_exportContext test1_export2_len test1_export2_exportValue in *)
+  (* let exp_res3 = test_export test1_ciphersuite test1_key test1_nonce test1_exporterSecret test1_export3_exportContext test1_export3_len test1_export3_exportValue in *)
+  (* let exp_res4 = test_export test1_ciphersuite test1_key test1_nonce test1_exporterSecret test1_export4_exportContext test1_export4_len test1_export4_exportValue in *)
 
-  let cs1 = test1_ciphersuite in
-  assert_norm (List.Tot.length test1_info <= HPKE.max_info);
-  assert_norm (List.Tot.length test1_skR == HPKE.size_dh_key cs1);
-  assert_norm (List.Tot.length test1_skI == HPKE.size_dh_key cs1);
-  assert_norm (List.Tot.length test1_skE == HPKE.size_dh_key cs1);
-//  assert_norm (List.Tot.length test1_pskID <= HPKE.max_pskID);
-  assert_norm (List.Tot.length test1_pkR == HPKE.size_dh_public cs1);
-  assert_norm (List.Tot.length test1_pkI == HPKE.size_dh_public cs1);
-  assert_norm (List.Tot.length test1_pkE == HPKE.size_dh_public cs1);
-  assert_norm (List.Tot.length test1_zz == HPKE.size_dh_public cs1);
-  // assert_norm (List.Tot.length test1_context == 7 + 3 * HPKE.size_dh_public cs1 + 2 * Hash.size_hash (HPKE.hash_of_cs cs1));
-
-  assert_norm (List.Tot.length test1_key == HPKE.size_aead_key cs1);
-  assert_norm (List.Tot.length test1_nonce == HPKE.size_aead_nonce cs1);
-
-  let res1 = test_base_setup cs1 test1_info test1_skR test1_skI test1_skE test1_psk test1_pskID
-    test1_pkR test1_pkI test1_pkE test1_enc test1_zz test1_context test1_secret test1_key test1_nonce in
-
-  assert_norm (List.Tot.length test1_cipher0 == 45);
-  assert_norm (List.Tot.length test1_plaintext == 29);
-  assert_norm (List.Tot.length test1_aad0 <= HPKE.max_info);
-
-  // Cannot be called because Vale has assumed functions in its AES-GCM spec, and
-  // tests on the implementation instead
-  // let res_encrypt0 = test_encrytion cs1 test1_skE test1_skR test1_pkR test1_pkE test1_plaintext
-  //   test1_aad0 test1_cipher0 in
-
-  res1 // && res_encrypt0
+  // TODO test encryption, or at least the nonce computation
+  enc_res0 (* && enc_res1 && enc_res2 && enc_res3 && enc_res4 && enc_res5 && enc_res6 && enc_res7 && enc_res8 && enc_res9*) && res && exp_res0 (* && exp_res1 && exp_res2 && exp_res3 && exp_res4 *)
 
 
-let test2 () =
-  IO.print_string "\nTest 2\n";
+(* let test1 () = *)
+(*   IO.print_string "\nTest 1\n"; *)
 
-  let cs2 = test2_ciphersuite in
+(*   let cs1 = test1_ciphersuite in *)
+(*   assert_norm (List.Tot.length test1_info <= HPKE.max_info); *)
+(*   assert_norm (List.Tot.length test1_skR == HPKE.size_dh_key cs1); *)
+(*   assert_norm (List.Tot.length test1_skI == HPKE.size_dh_key cs1); *)
+(*   assert_norm (List.Tot.length test1_skE == HPKE.size_dh_key cs1); *)
+(* //  assert_norm (List.Tot.length test1_pskID <= HPKE.max_pskID); *)
+(*   assert_norm (List.Tot.length test1_pkR == HPKE.size_dh_public cs1); *)
+(*   assert_norm (List.Tot.length test1_pkI == HPKE.size_dh_public cs1); *)
+(*   assert_norm (List.Tot.length test1_pkE == HPKE.size_dh_public cs1); *)
+(*   assert_norm (List.Tot.length test1_zz == HPKE.size_dh_public cs1); *)
+(*   // assert_norm (List.Tot.length test1_context == 7 + 3 * HPKE.size_dh_public cs1 + 2 * Hash.size_hash (HPKE.hash_of_cs cs1)); *)
 
-  assert_norm (List.Tot.length test2_info <= HPKE.max_info);
-  assert_norm (List.Tot.length test2_skR == HPKE.size_dh_key cs2);
-  assert_norm (List.Tot.length test2_skI == HPKE.size_dh_key cs2);
-  assert_norm (List.Tot.length test2_skE == HPKE.size_dh_key cs2);
+(*   assert_norm (List.Tot.length test1_key == HPKE.size_aead_key cs1); *)
+(*   assert_norm (List.Tot.length test1_nonce == HPKE.size_aead_nonce cs1); *)
 
-  assert_norm (List.Tot.length test2_pkR == HPKE.size_dh_public cs2);
-  assert_norm (List.Tot.length test2_pkI == HPKE.size_dh_public cs2);
-  assert_norm (List.Tot.length test2_pkE == HPKE.size_dh_public cs2);
-//  assert_norm (List.Tot.length test2_zz == HPKE.size_dh_public cs2);
+(*   let res1 = test_base_setup cs1 test1_info test1_skR test1_skI test1_skE test1_psk test1_pskID *)
+(*     test1_pkR test1_pkI test1_pkE test1_enc test1_zz test1_context test1_secret test1_key test1_nonce in *)
 
-  true
+(*   assert_norm (List.Tot.length test1_cipher0 == 45); *)
+(*   assert_norm (List.Tot.length test1_plaintext == 29); *)
+(*   assert_norm (List.Tot.length test1_aad0 <= HPKE.max_info); *)
+
+(*   // Cannot be called because Vale has assumed functions in its AES-GCM spec, and *)
+(*   // tests on the implementation instead *)
+(*   // let res_encrypt0 = test_encrytion cs1 test1_skE test1_skR test1_pkR test1_pkE test1_plaintext *)
+(*   //   test1_aad0 test1_cipher0 in *)
+
+(*   res1 // && res_encrypt0 *)
+
+
+(* let test2 () = *)
+(*   IO.print_string "\nTest 2\n"; *)
+
+(*   let cs2 = test2_ciphersuite in *)
+
+(*   assert_norm (List.Tot.length test2_info <= HPKE.max_info); *)
+(*   assert_norm (List.Tot.length test2_skR == HPKE.size_dh_key cs2); *)
+(*   assert_norm (List.Tot.length test2_skI == HPKE.size_dh_key cs2); *)
+(*   assert_norm (List.Tot.length test2_skE == HPKE.size_dh_key cs2); *)
+
+(*   assert_norm (List.Tot.length test2_pkR == HPKE.size_dh_public cs2); *)
+(*   assert_norm (List.Tot.length test2_pkI == HPKE.size_dh_public cs2); *)
+(*   assert_norm (List.Tot.length test2_pkE == HPKE.size_dh_public cs2); *)
+(* //  assert_norm (List.Tot.length test2_zz == HPKE.size_dh_public cs2); *)
+
+(*   true *)
 
 let test () =
-  let r1 = test1 () in
-  let r2 = test2 () in
-  r1 && r2
+  let r0 = test1 () in
+  (* let r1 = test1 () in *)
+  (* let r2 = test2 () in *)
+  (* r1 && r2 *)
+  r0
